# 10.2: Rational Exponents; From Radicals (Roots) to Rational Exponents

**What is Rational In Mathematics?**

When we refer to the word "Rational" in Mathematics, this means "ratio" or
"fraction". Thusly when we refer to rational exponents, we are referring to
exponents that are fractions.

- Any root can be represented as a _Rational Exponent_.

$$ \sqrt[n]{a} = a^{\frac{1}{n}}$$

**Ex:**

$$ 25^{\frac{1}{2}} = \sqrt[2]{25^1} = \sqrt{25} = 5 $$

$$ 27^{\frac{1}{3}} = \sqrt[3]{27} = 3 $$

$$ x^{\frac{1}{5}} = \sqrt[5]{x} $$

$$ -25^{\frac{1}{2}} = -1(25^{1/2}) = -1(\sqrt{25}) = -5 $$

Note the use of parentheses in the expression below:

$$ (-27y^6)^{\frac{1}{3}} = \sqrt[3]((-27^2)^3) = -3^2 $$

This is necessary of we want to include whatever is in the parentheses to the
power of, in this case, $\frac{1}{3}$. Notice how the following doesn't have
parentheses, thusly the 7 is considered a multiplier of the radicand, not part
of the radicand itself:

$$ 7x^{\frac{1}{5}} = 7(x^{\frac{1}{5}}) = 7\sqrt[5]{x} $$

This is as opposed to if we include the $7$ in the radicand using parentheses:

$$ (7x)^{\frac{1}{5}} = \sqrt[5]{7x} $$

---

**Ex:**

$$ x^{\frac{1}{4}} $$

$$ x^{\frac{1}{4}} = \sqrt[4]{x} $$

$$ -9^{\frac{1}{2}} = -1(9^{\frac{1}{2}}) = -\sqrt{9} = -3 $$

$$ (81x^8)^{\frac{1}{4}} = \sqrt[4]{81x^8} = \sqrt[4]{(81x^2)^4} = 3x^2 $$

$$ 5y^{\frac{1}{3}} $$

$$ 5y^{\frac{1}{3}} = 5\sqrt[3]{y}$$

---

So far, we have only ever had the radicand's power to $1$, but in fact, this can
be represented by another variable $m$:

$$ \sqrt[n]{a^m} = a^{\frac{m}{n}} $$

This can also be expressed as the following, albeit it is somewhat unintuitive:

$$ \sqrt[n]{a^m} = (\sqrt[n]{a})^m = (a^{\frac{1}{n}})^m = a^{\frac{1}{n}\times\frac{m}{1}} = a^{\frac{m}{n}} $$

This is because the way multiplication of exponents works.

---

**Ex:**

As an example, can we take the following and express it as a rational exponent?:

$$ \sqrt[3]{2^5} $$

$$ \sqrt[3]{2^5} = 2^{\frac{5}{3}}$$

Let's suppose we have a rational exponent, can we express that as a nth root?:

$$ 9^{\frac{3}{2}} $$

$$ 9^{\frac{3}{2}} = \sqrt[2]{9^3} = \sqrt{9^3} = \sqrt{729} = 27 $$

Though the above is rather cumbersome, and there is a shortcut:

$$ 9^{\frac{3}{2}} = (\sqrt{9})^3 = 3^3 = 27 $$

---

**Ex:**

$$ -256^{\frac{3}{4}} $$

$$ -256^{\frac{3}{4}} = -\sqrt[4]{256^3} = -(\sqrt[4]{256})^3 = -4^3 = -64 $$

$$ (-32)^{\frac{2}{5}} $$

$$ (-32)^{\frac{2}{5}} = \sqrt[5]{-32^2} = (\sqrt[5]{-32})^2 = -2^2 = 4 $$

---

Let's now move onto a fraction to the power of a fraction:

**Ex:**

$$ (\frac{1}{4})^{\frac{3}{2}} $$

$$ (\frac{1}{4})^{\frac{3}{2}} = \sqrt{(\frac{1}{4})^3} = (\sqrt{\frac{1}{4}})^3 = (\frac{1}{2})^3 = \frac{1}{8} $$

**Ex:**

$$ (2x+1)^{\frac{2}{7}} $$

$$ (2x+1)^{\frac{2}{7}} = \sqrt[7]{(2x+1)^2} $$

---

$$ -81^{\frac{3}{4}} $$

$$ -81^{\frac{3}{4}} = -\sqrt[4]{(81)^3} = -(\sqrt[4]{81})^3 = -3^3 = -27 $$

---

**Negative Exponents**

$$ a^{-1} = \frac{1}{a} $$

This is the same as:

$$ \frac{a}{1}^{-1} = \frac{1}{a} $$

$$ a^{-\frac{m}{n}} = \frac{1}{a^{\frac{m}{n}}} $$

Note that this does _not_ affect the sign of the number, just the sign of the
exponent.

Let's now work with some examples:

$$ 3^{-2} $$

$$ 3^{-2} = \frac{1}{3^2} $$

$$ 9^{-\frac{1}{2}} $$

$$ 9^{-\frac{1}{2}} = \frac{1}{9^{\frac{1}{2}}} = \frac{1}{3} $$

$$ 27^{-\frac{2}{3}} $$

$$ 27^{-\frac{2}{3}} = \frac{1}{27^{\frac{2}{3}}} = \frac{1}{3^2} = \frac{1}{9} $$

$$ -256^{-\frac{3}{4}} $$

$$ -256^{-\frac{3}{4}} = -\frac{1}{256^{\frac{3}{4}}} = \frac{1}{\sqrt[4]{256^3}} = \frac{1}{(\sqrt[4]{256})^3} = -\frac{1}{4^3} = -\frac{1}{64} $$

---

**Rules of Rational Exponents:**

1.

$$ a^m \times a^n = a^{m+n} $$

$$ x^2 \times x^3 = x^5 $$

2.

$$ (a^m)^n = a^{m\times n} $$

$$ (y^4)^3 = y^{12} $$

3.

$$ (ab)^m = a^mb^m $$

$$ (xy)^3 = x^3y^3 $$

$$ (a+b)^m \neq a^m + b^m $$

4.

$$ (\frac{a}{b})^m = \frac{a^m}{b^m} $$

$$ (\frac{3}{x}^2) = \frac{3^2}{x^2} = \frac{9}{x^2} $$

5.

$$ \frac{a^m}{a^n} = a^{m - n} $$

$$ \frac{y^2}{y^5} = y^{2-5} = y^{-3} = \frac{1}{y^3} $$

6.

$$ \frac{a}{0} = 1 $$

7.

$$ a^{-n} = \frac{1}{a^n} $$

$$ x^{-4} = \frac{1}{x^4} $$

---

**Ex:**

$$ x^{\frac{1}{3}} \times x^{\frac{1}{4}} = x^{\frac{1}{3} + \frac{1}{4}} =
x^{\frac{4}{12} + \frac{3}{12}}  = x^{\frac{7}{12}} = \sqrt[12]{x^7} $$

---

**Ex:**

$$ \frac{9^{\frac{2}{5}}}{9^{\frac{12}{5}}} = 9^{\frac{2}{5} - \frac{12}{5}}  =
9^{-\frac{10}{5}} = 9^{-2} = \frac{1}{9^2} = \frac{1}{81} $$

---

**Ex:**

$$ y^{\frac{-3}{10}} \times y^{\frac{6}{10}} = y^{\frac{-3}{10} + \frac{6}{10}} = y^{\frac{3}{10}} = \sqrt[10]{y^3} $$

---

**Ex:**

$$ (11^{\frac{2}{9}})^3 $$

$$ (11^{\frac{2}{9}})^3 = 11^{\frac{2}{9} \times 3} = 11^{\frac{6}{9}} =
11^{\frac{2}{3}} = \sqrt[3]{11^2} $$

---

**Ex:**

$$ \frac{(3x^{-\frac{2}{3}})^3}{x^2} $$

Let's first break this down according to the _Order of Operations_, which says
we must first address the parentheses:

$$ (3x^{-\frac{2}{3}})^3 = 3^3 \times x^{-\frac{2}{3} \times 3} = 3^3 \times
x^{-\frac{6}{3}} = 3^3 \times x^{-2} $$

This leaves our overall fraction currently at:

$$ \frac{3^3 \times x^{-2}}{x^2} $$

We have options to solve it at this point, we could simply take our numerator
multiplier, $x^{-2}$, and move it to the denominator by simply flipping the sign
of our exponent:

$$ \frac{3^3}{x^2 \times x^2} $$

And then we simplify:

$$ \frac{27}{x^4} $$

---

Practice:

$$ y^{\frac{2}{3}} \times y^{\frac{8}{3}} $$

$$ y^{\frac{2}{3}} \times y^{\frac{8}{3}} = y^{\frac{2}{3} + \frac{8}{3}} =
y^{\frac{10}{3}} = \sqrt[3]{y^{10}} $$

---

Practice:

$$ \frac{5^{\frac{1}{7}}}{5^{\frac{8}{7}}} = 5^{\frac{1}{7} - \frac{8}{7}} =
5^{\frac{-7}{7}} = 5^{-1} = \frac{1}{5} $$

---

Practice:

$$ x^{\frac{4}{9}} \times x^{-\frac{2}{9}} = x^{\frac{4}{9} + (-\frac{2}{9})} =
x^{\frac{2}{9}} = \sqrt[9]{x^2} $$

---

Practice:

$$ \frac{(3x^{\frac{1}{4}}y^{-\frac{2}{3}})^4}{x^4y} $$

Let's ignore the denominator for now:

$$ (3x^{\frac{1}{4}}y^{-\frac{2}{3}})^4 $$

$$ (3x^{\frac{1}{4}}y^{-\frac{2}{3}})^4 = 3^4x^{\frac{1}{4} \times 4}y^{-\frac{2}{3} \times 4} = 3^4xy^{-\frac{8}{3}} $$

Let's now take this simplified numerator and plug it into our starting fraction:

$$ \frac{3^4xy^{-\frac{8}{3}}}{x^4y} $$

$$ 3^4x^{1-4}y^{-\frac{8}{3} - 1} $$

$$ 3^4x^{-3}y^{-\frac{11}{3}} $$

$$ \frac{3^4}{x^3y^{\frac{11}{3}}} $$

---

Pretty good. But what about this example?:

$$ x^{\frac{3}{4}}(x^{\frac{1}{4}} - x^3) $$

This might seem overwhelming, but let's first look at a more simple example:

$$ x^3(x - x^3) $$

Let's first distribute our first $x^3$ to both of our terms inside of the
parentheses:

$$ (x^3 \times x) - (x^3 \times x^3) $$

Now we simplify by adding our bases:

$$ x^4 - x^6 $$

Knowing this, we can return to our original problem and apply the same
principle:

$$ x^{\frac{3}{4}}(x^{\frac{1}{4}} - x^3) $$

$$ (x^{\frac{3}{4}} \times x^{\frac{1}{4}}) - (x^{\frac{3}{4}} \times x^3) $$

$$ x - (x^{\frac{3}{4}} \times x^{\frac{12}{4}}) $$

$$ x - x^{\frac{15}{4}} $$

---

**Ex:**

$$ (x^{\frac{1}{4}} + 1)(x^{\frac{1}{4}} - 7) $$

$$ x^{\frac{2}{4}} - 6x^{\frac{1}{4}} - 7 $$

$$ x^{\frac{1}{2}} - 6x^{\frac{1}{4}} - 7 $$

---

**Practice:**

$$ x^{\frac{3}{5}}(x^{\frac{1}{3}} - x^2) $$

$$ (x^{\frac{3}{5}} \times x^{\frac{1}{3}}) - (x^{\frac{3}{5}} \times x^2) $$

$$ (x^{\frac{9}{15}} \times x^{\frac{5}{15}}) - (x^{\frac{3}{5}} \times x^{\frac{10}{5}}) $$

$$ x^{\frac{14}{15}} - x^{\frac{13}{5}} $$

---

**Practice:**

$$ (x^{\frac{1}{2}}+6)(x^{\frac{1}{2}}-2) $$

$$ (x^{\frac{1}{2}} \times x^{\frac{1}{2}}) + (6x^{\frac{1}{2}} - 2x^{\frac{1}{2}}) + (6 \times -2)$$

$$ x + 4x^{\frac{1}{2}} - 12 $$

---

**Factoring Using Rational Exponents:**

- We're going to _Factor_ $x^{-\frac{1}{3}}$ from
  $7x^{-\frac{1}{3}} - 5x^{\frac{5}{3}}$

Before, let's review more basic factoring:

Factor $x^2$ from $3x^2 - 10x^5$.

Recall that _Factoring_ is the _Opposite_ of _Distributing_x.

Thusly if we _Multiply_ when we _Distribute_, then we _Divide_ when _Factoring_:

$$ 3x^2 - 10x^5 = x^2(3 - 10x^3) $$

Let's now return to our original problem with this in mind:

- We're going to _Factor_ $x^{-\frac{1}{3}}$ from
  $7x^{-\frac{1}{3}} - 5x^{\frac{5}{3}}$

Thusly we can start our expression of factoring like:

$$ x^{-\frac{1}{3}}() $$

Continuing on, we can factor like with our more simple example:

$$ x^{-\frac{1}{3}}(7 - 5x^{\frac{5}{3} - (-\frac{1}{3})}) $$

$$ x^{-\frac{1}{3}}(7 - 5x^{\frac{5}{3} + \frac{1}{3}}) $$

$$ x^{-\frac{1}{3}}(7 - 5x^{\frac{6}{3}}) $$

$$ x^{-\frac{1}{3}}(7 - 5x^2) $$

---

**Practice:**

Factor $x^{-\frac{1}{5}}$ out of $2x^{-\frac{1}{5}} - 7x^{\frac{4}{5}}$:

$$ x^{-\frac{1}{5}}(2x^{-\frac{1}{5} - (-\frac{1}{5})} - 7x^{\frac{4}{5} - (-\frac{1}{5})}) $$

$$ x^{-\frac{1}{5}}(2x^{-\frac{1}{5} +\frac{1}{5}} - 7x^{\frac{4}{5} + \frac{1}{5}}) $$

$$ x^{-\frac{1}{5}}(2x^0 - 7x^{\frac{5}{5}}) $$

$$ x^{-\frac{1}{5}}(2(1) - 7x^{1}) $$

$$ x^{-\frac{1}{5}}(2 - 7x) $$

---

Let's refresh our memory a bit, let's write a root as a fraction:

$$ \sqrt[10]{y^5} $$

$$ \sqrt[10]{y^5} = y^{\frac{5}{10}}$$

But if we simplify this further, we get:

$$ \sqrt[10]{y^5} = y^{\frac{5}{10}} = y^{\frac{1}{2}} $$

And we know that $y^{\frac{1}{2}}$ is the same as $\sqrt[2]{y}$ or $\sqrt{y}$:

$$ \sqrt[10]{y^5} = y^{\frac{5}{10}} = y^{\frac{1}{2}} = \sqrt{y}$$

---

Let's do that one more time:

$$ \sqrt[9]{a^6n^3} $$

Always remember the rule when expressing square roots as fractional exponents...

_Power Over Root_:

$$ \sqrt[9]{a^6n^3} = a^{\frac{6}{9}}n^{\frac{3}{9}} $$

And then we can simplify our fractional exponents:

$$ \sqrt[9]{a^6n^3} = a^{\frac{2}{3}}n^{\frac{1}{3}} $$

Because the denominator of both exponents are the same, we can then simplify the
original root expression by factoring out the denominator as a root:

$$ \sqrt[3]{a^2n} $$

Note that we're simply dividing the radicand's exponent's by the root. This is
made obvious when taking our original expression and placing it next to our
simplified expression:

$$ \sqrt[9]{a^6n^3} = \sqrt[3]{a^2n} $$

---

Let's try another one:

$$ \sqrt{y} \times \sqrt[3]{y} $$

Is there a way we can simplify this expression as _one root_?

Let's first try to express each of these root expressions as rational exponents:

$$ \sqrt{y} = y^{\frac{1}{2}} $$

and

$$ \sqrt[3]{y} = y^{\frac{1}{3}} $$

Then we multiply these new expressions as per our original expression:

$$ \sqrt{y} \times \sqrt[3]{y} = y^{\frac{1}{2}} \times y^{\frac{1}{3}} $$

Which we know, as per multiplication of exponents, we can add the exponents:

$$ y^{\frac{1}{2}} \times y^{\frac{1}{3}} = y^{\frac{1}{2} + \frac{1}{3}}$$

Then we convert them to the same denominator:

$$ y^{\frac{1}{2} + \frac{1}{3}} = y^{\frac{3}{6} + \frac{2}{6}}$$

Which evaluates to:

$$ y^{\frac{5}{6}} $$

Which we can express this as the simplified root:

$$ \sqrt[6]{y^5} $$
