# 10.3 Simplifying Radical (Roots)

Simplifying radicals works on 1 simple rule called _Product Rule_:

$$ \sqrt[n]{a \times b} = \sqrt[n]{a} \times \sqrt[n]{b} $$

For example

$$ \sqrt{36} = \sqrt{9 \times 4} = \sqrt{9} \times \sqrt{4} = 3 \times 2 = 6 $$

Note that this works in reverse as well:

$$ \sqrt{2} \times \sqrt{7} = \sqrt{2 \times 7} = \sqrt{14} $$

---

Not only does thiw work for square roots, it works for _any type of root._

$$ \sqrt[4]{6} \times \sqrt[4]{3x^2} $$

$$ \sqrt[4]{6} \times \sqrt[4]{3x^2} = \sqrt[4]{6 \times 3x^2} = \sqrt[4]{18x^2}$$

---

Let's take another example:

$$ \sqrt{\frac{3}{x}} \times \sqrt{\frac{y}{2}} $$

$$ \sqrt{\frac{3}{x}} \times \sqrt{\frac{y}{2}} = \sqrt{\frac{3}{x} \times \frac{y}{2}} = \sqrt{\frac{3y}{2x}} $$

---

Just as there is a _Product Rule_ for simplifying radicals, there is also a
_Quotient Rule_:

$$ \sqrt[n]{\frac{a}{b}} = \frac{\sqrt[n]{a}}{\sqrt[n]{b}}$$

---

**Ex:**

$$ \sqrt{\frac{9}{25}} = \frac{\sqrt{9}}{\sqrt{25}} = \frac{3}{5} $$

---

**Ex:**

$$ \sqrt{\frac{y}{36}} = \frac{\sqrt{y}}{\sqrt{36}} = \frac{\sqrt{y}}{6} $$

---

**Ex:**

This also works with a cube root:

$$ \sqrt[3]{\frac{27}{64}} = \frac{\sqrt[3]{27}}{\sqrt[3]{64}} = \frac{3}{4} $$

---

**Ex:**

$$ \sqrt[5]{\frac{7}{32x^5}} = \frac{\sqrt[5]{7}}{\sqrt[5]{32x^5}} = \frac{\sqrt[5]{7}}{2x} $$

---

So what is the _goal_ for simplifying radicals?

The goal for simplifying radicals is for looking for _perfect n<sup>th</sup>
roots_.

---

**Practice:**

$$ \sqrt{18} $$

When determining how to simplify this, you _could_ choose to divide it up into:

$$ \sqrt{18} = \sqrt{6} \times \sqrt{3} $$

But $6$ and $3$ are not part of the _Perfect Squares_ number set. Instead,
choosing numbers we can square (or at least one we can square), like $9$ and
$2$, we can better simplify our radical:

$$ \sqrt{18} = \sqrt{9 \times 2} = \sqrt{9} \times \sqrt{2} = 3\sqrt{2} $$

---

**Practice:**

$$ \sqrt{98} $$

$$ \sqrt{98} = \sqrt{49 \times 2} = \sqrt{49} \times \sqrt{2} = 7\sqrt{2} $$

---

**Ex:**

Take this example:

$$ \sqrt{32} $$

We could factor out $4$ from $32$, but then we would get this:

$$ \sqrt{32} = \sqrt{4 \times 8} = \sqrt{4} \times \sqrt{8} = 2\sqrt{8} $$

If we inspect this though, we recognize that we can still further factor out
_Perfect Square_ numbers from $8$, Thusly it continues on:

$$ \sqrt{32} = \sqrt{4 \times 8} = \sqrt{4} \times \sqrt{8} = 2\sqrt{8} =
2\sqrt{4 \times 2} = 2\times \sqrt{4} \times \sqrt{2} = 2\times 2 \times \sqrt{2} = 4\sqrt{2} $$

To avoid taking all these extra steps, try and _factor out the largest perfect
square_ number that you can:

$$ \sqrt{32} = \sqrt{16 \times 2} = \sqrt{16} \times \sqrt{2} = 4\sqrt{2} $$

---

**Ex:**

$$ \sqrt{14} $$

$$ \sqrt{14} = \sqrt{7 \times 2} = \sqrt{7}\sqrt{2} = \text{NOT ABLE TO BE FURTHER SIMPLIFIED}$$

---

**Ex:**

$$ \sqrt[3]{40} $$

Moving onto simplifying cube root radicals, we should recall our _Perfect Cube_
numbers:

$$ \text{PERFECT CUBES} = 1, 8, 27, 64, 125 $$

Knowing this, we can take these numbers and see which of them can factor $40$:

$$ \sqrt[3]{40} = \sqrt[3]{8 \times 5} $$

Then we can further simplify:

$$ \sqrt[3]{40} = \sqrt[3]{8 \times 5} = \sqrt[3]{8} \times \sqrt[3]{5} = 2\sqrt[3]{5} $$

---

**Practice:**

$$ \sqrt[3]{54} = \sqrt[3]{27 \times 2} = \sqrt[3]{27} \times \sqrt[3]{2} = 3\sqrt[3]{2} $$

---

**Practice:**

$$ \sqrt{81y^5} $$

$$ \sqrt{81y^5} = \sqrt{81 \times y^2 \times y^2 \times y^1} = 9 \times y \times y \times \sqrt{y} = 9y^2\sqrt{y} $$

---

$$ \sqrt[3]{24a^9b^4} $$

$$ \sqrt[3]{24a^9b^4} = \sqrt[3]{8 \times 3 \times a^3 \times a^3 \times a^3 \times b^3 \times b^1} = 2 \times \sqrt[3]{3} \times a \times a \times a \times b \times \sqrt[3]{b} = 2a^3b\sqrt[3]{3b} $$

---

**Practice:**

$$ \sqrt[4]{32x^7} $$

Let's look at perfect 4 roots:

$$ \text{PERFECT ROOT 4 NUMBERS} = 1, 16, 81, 256, 625 $$

$32$ is divisible by $16$, which is the largest from that set that we can factor
out of:

$$ \sqrt[4]{32x^7} = \sqrt[4]{16 \times 2 \times x^4 \times x^3 } = 2 \times \sqrt[4]{2} \times x \times \sqrt[4]{x^3}= 2x\sqrt[4]{2x^3} $$

---

**Practice:**

$$ \sqrt{36z^7} $$

$$ \sqrt{36^7} = \sqrt{9 \times 4 \times z^2 \times z^2 \times z^2 \times z^1} $$

$$ \sqrt{36^7} = 3 \times 2 \times z \times z \times z \times \sqrt{z} $$

$$ \sqrt{36^7} = 6z^3\sqrt{z} $$

---

**Practice:**

$$ \sqrt[3]{32x^4y^7} $$

$$ \text{PERFECT CUBES} = 1, 8, 27, 64, 125 $$

$$ \sqrt[3]{32x^4y^7} = \sqrt[3]{8 \times 4 \times x^3 \times x^1 \times y^3 \times y^3 \times y^1}$$

$$ \sqrt[3]{32x^4y^7} = 2 \times \sqrt[3]{4} \times x \times \sqrt[3]{x} \times y \times y \times \sqrt[3]{y} $$

$$ \sqrt[3]{32x^4y^7} = 2xy^2\sqrt[3]{4xy} $$

---

**Practice:**

**Note:** Always _Combine Roots First Before You Simplify_.

$$ \frac{\sqrt{75}}{\sqrt{3}} $$

Let's first simplify the numerator first:

$$ \sqrt{75} = \sqrt{25 \times 3} = \sqrt{25} \times \sqrt{3} = 5\sqrt{3} $$

Now returning this to the numerator position:

$$ \frac{5\sqrt{3}}{\sqrt{3}} = 5 $$

However, we can also simply do this due to the _Quotient Rule_:

$$ \frac{\sqrt{75}}{\sqrt{3}} = \sqrt{\frac{75}{3}} = \sqrt{25} = 5 $$

---

**Practice:**

$$ \frac{\sqrt{80y}}{3\sqrt{5}} $$

Let's again simplify the numerator first:

$$ \sqrt{80y} = \sqrt{16 \times 5 \times y} = 4 \times \sqrt{5} \times \sqrt{y} $$

We return this to our numerator, keeping the delineation between $\sqrt{5}$ and
$\sqrt{y}$ to ease further simplification:

$$ \frac{\sqrt{80y}}{3\sqrt{5}} = \frac{4\sqrt{5}\sqrt{y}}{3\sqrt{5}} $$

Simplifying finally to:

$$ \frac{\sqrt{80y}}{3\sqrt{5}} = \frac{4\sqrt{y}}{3} $$

Another way we can approach this problem, we can separate out our multipliers
from the roots like so:

$$ \frac{\sqrt{80y}}{3\sqrt{5}} = \frac{1}{3} \times \frac{\sqrt{80y}}{\sqrt{5}} $$

$$ \frac{\sqrt{80y}}{3\sqrt{5}} = \frac{1}{3} \times \sqrt{\frac{80y}{5}} $$

$$ \frac{\sqrt{80y}}{3\sqrt{5}} = \frac{1}{3}\sqrt{16y} $$

$$ \frac{\sqrt{80y}}{3\sqrt{5}} = \frac{1}{3} \times 4 \times \sqrt{y} $$

$$ \frac{\sqrt{80y}}{3\sqrt{5}} = \frac{4}{3}\sqrt{y} = \frac{4\sqrt{y}}{3} $$

---

**Practice:**

$$ \frac{5\sqrt[3]{162x^8}}{\sqrt[3]{3x^2}} $$

$$ \frac{5}{1} \times \frac{\sqrt[3]{162^8}}{\sqrt[3]{3x^2}} $$

Because of the _Quotient Rule_, we can further simplify the expression to:

$$ 5\sqrt[3]{\frac{162x^8}{3x^2}} $$

$$ 5\sqrt[3]{\frac{54x^8}{x^2}} $$

$$ 5\sqrt[3]{54x^{8-2}} $$

$$ 5\sqrt[3]{54x^6} $$

$$ \text{PERFECT CUBES} = 1, 8, 27, 64, 125 $$

$$ 5\sqrt[3]{27 \times 2 \times x^3 \times x^3} $$

$$ 5 \times 3 \times \sqrt[3]{2} \times x \times x $$

$$ 15x^2\sqrt[3]{2} $$

---

**Practice:**

$$ \frac{3\sqrt[4]{32x^9y^6}}{\sqrt[4]{x^{-3}y}} $$

$$ \frac{3}{1} \times \frac{\sqrt[4]{32x^9y^6}}{\sqrt[4]{x^{-3}y}} $$

$$ \frac{3}{1} \times \sqrt[4]{\frac{32x^9y^6}{x^{-3}y}}$$

$$ \frac{3}{1} \times \sqrt[4]{32x^{12}y^5}$$

$$ \text{PERFECT ROOT 4 NUMBERS} = 1, 16, 81, 256, 625 $$

$$ \frac{3}{1} \times \sqrt[4]{16 \times 2 \times x^4 \times x^4 \times x^4 \times y^4 \times y^1} $$

$$ \frac{3}{1} \times 2 \times \sqrt[4]{2} \times x \times x \times x \times y \times \sqrt[4]{y} $$

$$ \frac{3}{1} \times 2x^3y\sqrt[4]{2y} $$

$$ 6x^3y\sqrt[4]{2y} $$

---

**Practice:**

$$ \frac{\sqrt[3]{40x^5y^7}}{5\sqrt[3]{5x^{-1}y^2}} $$

$$ \frac{1}{5} \times \frac{\sqrt[3]{40x^5y^7}}{\sqrt[3]{5x^{-1}y^2}} $$

$$ \frac{1}{5} \times \sqrt[3]{\frac{40x^5y^7}{5x^{-1}y^2}} $$

$$ \frac{1}{5} \times \sqrt[3]{8x^6y^5} $$

$$ \frac{1}{5} \times \sqrt[3]{2^3 \times x^3 \times x^3 \times y^3 \times y^2} $$

$$ \frac{1}{5} \times 2 \times x \times x \times y \times \sqrt[3]{y^2} $$

$$ \frac{1}{5} \times 2x^2y\sqrt[3]{y^2} $$

$$ \frac{2x^2y\sqrt[3]{y^2}}{5} $$
