# 10.7 An Introduction to Operations with Complex Numbers

Consider this:

> Is $\sqrt{-9}$ possible?

Technically we have not covered the nuance behind the answer. Let's rephrase the
question:

> Is $\sqrt{-9}$ possible to represent as a _Real Number_?

And the answer is _no_.

Today, however, we will introduce the concept of _Imaginary Numbers_. Now,
contrary to it's name, _Imaginary Numbers_ are not "imaginary" in the
traditional sense of the word, but the word _Imaginary_ here simply indicates
that they are the _opposite_ of _Real Numbers_.

---

**Imaginary Numbers:**

In order to deal with our $\sqrt{-9}$ from before, really we only have to
address one form of the same statement:

$$ \sqrt{-1} $$

We can define $\sqrt{-1}$ as the _Number_ $i$?:

$$ i = \sqrt{-1} $$

Now, we know that we can simplify roots by taking them to the power of the root:

$$ (i)^2 = (\sqrt{-1})^2 $$

$$ i^2 = -1 $$

This allows us to _rewrite_ the square roots of _negative_ numbers:

---

**Ex:**

$$ \sqrt{-9} = \sqrt{-1 \times 9} = \sqrt{-1} \times \sqrt{9} = 3i $$

---

**Ex:**

$$ \sqrt{-25} = \sqrt{-1 \times 25} = \sqrt{-1} \times \sqrt{25} = 5i $$

---

**Ex:**

$$ \sqrt{-3} = \sqrt{-1 \times 3} = \sqrt{-1} \times \sqrt{3} = i\sqrt{3} $$

---

**Ex:**

$$ -\sqrt{-50} = -(\sqrt{-1 \times 50}) = -(\sqrt{-1 \times 2 \times 25}) = -(\sqrt{-1} \times \sqrt{2} \times \sqrt{25}) = -(5\sqrt{-1}\sqrt{2}) = -5i\sqrt{2} $$

$$ -5i\sqrt{2} $$

---$a

**Ex:**

$$ \sqrt{-7} $$

$$ \sqrt{-7} = \sqrt{-1 \times 7} $$

$$ \sqrt{-7} = i\sqrt{7} $$

---

**Ex:**

$$ -\sqrt{-18} $$

$$ -\sqrt{-18} = -(\sqrt{-1 \times 18}) $$

$$ -\sqrt{-18} = -(\sqrt{-1} \times \sqrt{18}) $$

$$ -\sqrt{-18} = -(\sqrt{-1} \times \sqrt{9} \times \sqrt{2}) $$

$$ -\sqrt{-18} = -(i \times 3 \times \sqrt{2}) $$

$$ -\sqrt{-18} = -3i\sqrt{2} $$

---

**Ex:**

$$ \sqrt{-2} \times \sqrt{-7} $$

Notice, with our knowledge of $i$, we have two ways of solving this. We could
simply multiply $-2$ by $-7$ within our root:

$$ \sqrt{-2 \times -7} $$

$$ \sqrt{-2 \times -7} = \sqrt{14} $$

But, if we solve this, knowing that _when we have a negative radicand_, we must
represent these radicals as imaginary numbers. Indeed, if we treat these radical
numbers appropriately by calculating them with $i$ in mind, we get a different
answer:

$$ \sqrt{-2} = \sqrt{-1 \times 2} $$

$$ \sqrt{-2} = \sqrt{-1} \times \sqrt{2} $$

$$ \sqrt{-2} = i \times \sqrt{2} $$

$$ \sqrt{-2} = i\sqrt{2} $$

$$ \sqrt{-7} = \sqrt{-1 \times 7} $$

$$ \sqrt{-7} = \sqrt{-1} \times \sqrt{7} $$

$$ \sqrt{-7} = i \times \sqrt{7} $$

$$ \sqrt{-7} = i\sqrt{7} $$

$$ i\sqrt{2} \times i\sqrt{7} $$

$$ i^2\sqrt{2}\sqrt{7} $$

$$ i^2\sqrt{2 \times 7} $$

$$ i^2\sqrt{14} $$

$$ -1\sqrt{14} $$

$$ -\sqrt{14} $$

This proves that another rule of $i$ is that $i^2$ is equal to $-1$:

$$ i^2 = -1 $$

Thusly we have two rules for $i$:

$$ i = \sqrt{-1} $$

$$ i^2 = -1 $$

Finally, we can see that we get two different answers:

$$ \sqrt{14} \neq -\sqrt{14} $$

Our original, implementation does not apply when imaginary numbers are involved.
Thusly _if you see a radical negative number, you CANNOT apply the rule of
multiplication to it._ To be clear, the actual answer to our problem is:

$$ -\sqrt{14} $$

---

**Ex:**

$$ \sqrt{-25} \times \sqrt{-1} $$

$$ \sqrt{-25} = \sqrt{-1 \times 25} $$

$$ \sqrt{-25} = \sqrt{-1} \times \sqrt{25} $$

$$ \sqrt{-25} = i \times 5 $$

$$ \sqrt{-25} = 5i $$

$$ 5i \times i $$

$$ 5i^2 $$

$$ -5 $$

---

$$ \sqrt{27} \times \sqrt{-3} $$

$$ \sqrt{-3} = \sqrt{-1 \times 3}$$

$$ \sqrt{-3} = \sqrt{-1} \times \sqrt{3}$$

$$ \sqrt{-3} = i\sqrt{3}$$

$$ \sqrt{27} \times i\sqrt{3} $$

$$ \sqrt{9 \times 3} \times i\sqrt{3} $$

$$ \sqrt{9} \times \sqrt{3} \times i\sqrt{3} $$

$$ 3\sqrt{3} \times i\sqrt{3} $$

$$ 3i(\sqrt{3})^2 $$

$$ 3i(3) $$

$$ 9i $$

---

**Ex:**

$$ \frac{\sqrt{-8}}{\sqrt{2}} $$

$$ \sqrt{-8} = \sqrt{-1 \times 8} $$

$$ \sqrt{-8} = \sqrt{-1} \times \sqrt{8} $$

$$ \sqrt{-8} = i \times \sqrt{4 \times 2} $$

$$ \sqrt{-8} = i \times \sqrt{4} \times \sqrt{2} $$

$$ \sqrt{-8} = i \times 2 \times \sqrt{2} $$

$$ \sqrt{-8} = 2i\sqrt{2} $$

$$ \frac{2i\sqrt{2}}{\sqrt{2}} $$

$$ 2i $$

---

**Ex:**

$$ \sqrt{-5} \times \sqrt{-6} $$

$$ \sqrt{-5} = \sqrt{-1} \times \sqrt{5} $$

$$ \sqrt{-5} = i\sqrt{5} $$

$$ \sqrt{-6} = \sqrt{-1} \times \sqrt{6} $$

$$ \sqrt{-6} = i\sqrt{6} $$

$$ i\sqrt{5} \times i\sqrt{6} $$

$$ i^2\sqrt{5 \ times 6} $$

$$ i^2\sqrt{30} $$

$$ -\sqrt{30} $$

---

**Ex:**

$$ \frac{\sqrt{-27}}{\sqrt{3}} $$

$$ \sqrt{-27} = 3i\sqrt{3} $$

$$ \frac{3i\sqrt{3}}{\sqrt{3}} $$

$$ 3i $$

---

**Complex Numbers:**

_Imaginary Numbers_ are really just a subtype of a larger group of numbers known
as _Complex Numbers_. By pairing a _Real Number_ with an _Imaginary Number_, we
create a _Complex Number_.

A complex number can take this form:

$$ a + bi $$

$$ a =  \text{REAL PART} $$

$$ bi = \text{IMAGINARY PART} $$

To give you an idea of the scope of _Complex Numbers_, please try to comprehend
that _Real Numbers_ include all conceivable (and inconceivable) numbers between
$-\infty$ and $\infty$, including all decimal numbers (3.7), irrational
numbers(3.333333...), $\pi$, etc.

Then, when combining infinite scope of _Real Numbers_ with the infinite set that
there are of _Imaginary Numbers_, we get the incredibly vast large scope
_Complex Numbers_. This effectively makes the scope of _Complex Numbers_ to be
$2\infty$.

Technically, this means that _All Numbers Are Automaticallly Complex Numbers_!!

**Ex:**

$$ 7 = 7 + 0i $$

$$ 3i = 0 + 3i $$

---

**Adding and Subtracting Complex Numbers:**

**Ex:**

$$ (5 + 2i) + (4 - 3i) $$

The parentheses here are there solely to emphasize that each expression wrapped
in parentheses represents a single _Complex Number_.

$$ (5 + 2i) = \text{A COMPLEX NUMBER} $$

$$ (4 - 3i) = \text{A COMPLEX NUMBER} $$

Now, we can simply treat this as a standard PEMDAS expression:

$$ 5 + 2i + 4 - 3i $$

And combine like terms:

$$ 9 - i $$

**Ex:**

$$ 6i - (2 - i) $$

$$ 6i - 2 + i $$

$$ 7i - 2 $$

But note we _cannot_ represent a _Complex Number_ in this form, since we are
dealing in _Complex Numbers_, we should write it in the proper form:

$$ -2 + 7i $$

---

**Ex:**

$$ (-2 - 4i) - (-3 + i) $$

$$ -2 - 4i + 3 - i $$

$$ 1 - 5i $$

---

**Practice:**

$$ (3 - 5i) + (-4 + i) $$

$$ 3 - 5i - 4 + i $$

$$  -1 - 4i $$

---

**Practice:**

$$ (-5 - 2i) - (-8 - 4i) $$

$$ -5 - 2i + 8 + 4i $$

$$ 3 + 2i $$

---

$$ (4 - \sqrt{-25}) - (-3 + \sqrt{-4}) $$

$$ sqrt{-25} = 5i $$

$$ \sqrt{-4} = 2i $$

$$ (4 - 5i) - (-3 + 2i) $$

$$ 4 - 5i + 3 - 2i $$

$$ 7 - 7i $$

---

**Multiply**

When multiplying complex numbers, just remember this:

$$ i^2 = -1 $$

**Ex:**

$$ -5i \times 3i $$

$$ -15i^2 $$

$$ -15(-1) $$

$$ 15 $$

---

**Ex:**

$$ -3i(6 - 2i) $$

$$ (-3i)(6) + (-3i)(-2i) $$

$$ -18i + 6i^2 $$

$$ -18i + 6(-1) $$

$$ -18i - 6 $$

$$ -6 - 18i $$

---

**Practice:**

$$ (3 - 4i)(6 + i) $$

$$ (3)(6) - (4i)(6) + 3i - 4i^2 $$

$$ 18 - 24i + 3i - 4i^2 $$

$$ 18 - 21i - 4i^2 $$

$$ 18 - 21i - 4(-1) $$

$$ 18 - 21i + 4 $$

$$ 22 - 21i $$

---

**Practice:**

$$ (1 - 2i)^2 $$

$$ (1 - 2i)(1 - 2i) $$

$$ (1)(1) - (2i)(1) - (2i)(1) + (2i)(2i) $$

$$ 1 - 2i - 2i + 4i^2 $$

$$ 1 - 4i + 4i^2 $$

$$ 1 - 4i + 4(-1) $$

$$ 1 - 4i - 4 $$

$$ -3 - 4i $$

---

**Ex:**

$$ (6 + 5i)(6 - 5i) $$

$$ (6)(6) + (5i)(6) - (5i)(6) - (5i)(5i) $$

$$ 36 - 25i^2 $$

$$ 36 - 25(-1) $$

$$ 36 + 25 $$

$$ 61 $$

---

**Practice:**

$$ -4i \times 5i $$

$$ -20i^2 $$

$$ -20(-1) $$

$$ 20 $$

---

**Practice:**

$$ (2 + 3i)(6 - i) $$

$$ (2)(6) + (3i)(6) - (2)(i) - (3i)(i) $$

$$ 12 + 18i - 2i - 3i^2 $$

$$ 12 + 16i - 3(-1) $$

$$ 12 + 16i + 3 $$

$$ 15 + 16i $$

---

**Practice:**

$$ (3 - i)^2 $$

$$ (3 - i)(3 - i) $$

$$ (3)(3) - (3)(i) - (3)(i) + (i)(i) $$

$$ 9 - 6i - 1 $$

$$ 8 - 6i $$

---

**Dividing:**

$$ \frac{3 + i}{2 - 3i} $$

To solve this, we can multiply by the _Conjugate_ of the denominator.

$$ \frac{3 + i}{2 - 3i} \times \frac{2 + 3i}{2 + 3i} $$

$$ \frac{(3 + i)(2 + 3i)}{(2 - 3i)(2 + 3i)} $$

$$ \frac{6 + 9i + 2i + 3i^2}{4 + 6i - 6i - 9i^2} $$

$$ \frac{6 + 11i + 3(-1)}{4 - 9(-1)} $$

$$ \frac{6 + 11i - 3}{4 + 9} $$

$$ \frac{3 + 11i}{13} $$

Note that to express this in the proper form for a _Complex Number_, we'll have
to now simply split it up to fit the proper form:

$$ \frac{3}{13} + \frac{11}{13}i $$

---

**Ex:**

$$ \frac{6}{5i} $$

This can be confusing, but keep in mind that we need to multiply by the
_Conjugate Number_, and _All Numbers are Coplex Numbers_. Thusly our expression
could also be expressed as this:

$$ \frac{6}{0 + 5i} $$

This allows us to determine the _Conjugate Number_:

$$ \frac{6}{5i} \times \frac{0 - 5i}{0 - 5i} $$

Or:

$$ \frac{6}{5i} \times \frac{-5i}{-5i} $$

This becomes:

$$ \frac{6(-5i)}{5i(-5i)} $$

$$ \frac{-30i}{-25i^2} $$

$$ \frac{-30i}{-25(-1)} $$

$$ \frac{-30i}{25} $$

$$ -\frac{6}{5}i $$

Which expressed as a complex number is:

$$ 0 - \frac{6}{5}i $$

---

**Practice:**

$$ \frac{4 - i}{3 + i} $$

$$ \frac{4 - i}{3 + i} \times \frac{3 - i}{3 - i} $$

$$ \frac{(4 - i)(3 - i)}{(3 + i)(3 - i)} $$

$$ \frac{4(3) - 3i - 4i + i^2}{9 + 3i - 3i - i^2} $$

$$ \frac{12 - 7i + (-1)}{9 - (-1)} $$

$$ \frac{11 - 7i}{10} $$

$$ \frac{11}{10} - \frac{7}{10}i $$

---

**Practice:**

$$ \frac{2}{3i} $$

$$ \frac{2}{3i} \times \frac{0 - 3i}{0 - 3i} $$

$$ \frac{2}{3i} \times \frac{-3i}{-3i} $$

$$ \frac{(2)(-3i)}{(3i)(-3i)} $$

$$ \frac{-6i}{-9i^2} $$

$$ \frac{-6i}{-9(-1)} $$

$$ \frac{-6i}{9} $$

$$ -\frac{2}{3}i $$

---

**The Powers of $i$**

$$ i^1 = i $$

$$ i^2 = -1 $$

$$ i^3 = i^2 \times i = -1 \times i = -i $$

$$ i^3 = -i $$

$$ i^4 = i^2 \times i^2 = -1 \times -1 = 1 $$

$$ i^4 = 1 $$

$$ i^5 = i^2 \times i^2 \times i = -1 \times -1 \times i = 1 \times i = i $$

Notice that we are now in an intriguing cycle, we are now getting into the realm
of _Number Theory_:

$$ i^5 = i^1 = i $$

$$ i^6 = i^2 = -1 $$

$$ i^7 = i^3 = -i $$

$$ i^7 = i^3 = -i $$

$$ i^8 = i^4 = 1 $$

$$ i^9 = i^1 = i $$

Now let's say we had $i$ to a large exponent power:

$$ i^50 $$

Obviously we wouldn't want to cycle through this multiple times to find our
answer, instead, a simple formula will give help us find the answer, simply take
the exponent and take the _modulo_ of the exponent divided by $4$ (the remainder
after dividing by $4$).

$$ 50\mod 4 = 2 $$

The remainder is the power we can reduce $i$ to in order to determine the value
of our $i$ to the power of the exponent, thusly:

$$ i^50 = i^{(50\mod 4)} = i^2 = -1 $$

Let's try it with another example:

$$ i^12 = i^{(12 \mod 4)} = i^0 = 1 $$

Recall that any number to the $0$<sup>th</sup> power is $1$.
