# 12.1 Operations and Composition of Functions

$$ (f + g)(x) = f(x) + g(x) $$

$$ (f - g)(x) = f(x) - g(x) $$

$$ (f \times g)(x) = f(x) \times g(x) $$

$$ (\frac{f}{g})(x) = \frac{f(x)}{g(x)}, g(x) \neq 0 $$

---

**Ex:**

$$ f(x) = x + 3, g(x) = 3x - 1 $$

$$ (f + g)(x) = (x + 3) + (3x - 1) $$

$$ (f + g)(x) = x + 3 + 3x - 1 $$

**Solution**:

$$ (f + g)(x) = 4x + 2 $$

---

**Ex:**

$$ f(x) = x + 3, g(x) = 3x - 1 $$

$$ (f - g)(x) = (x + 3) - (3x - 1) $$

$$ (f - g)(x) = x + 3 - 3x + 1 $$

**Solution**:

$$ (f - g)(x) = -2x + 4 $$

---

**Ex:**

$$ f(x) = x + 3, g(x) = 3x - 1 $$

$$ (f \times g)(x) = (x + 3) \times (3x - 1) $$

$$ (f \times g)(x) = (x + 3)(3x - 1) $$

$$ (f \times g)(x) = 3x^2 + 9x - x - 3 $$

**Solution**:

$$ (f \times g)(x) = 3x^2 + 8x - 3 $$

---

**Ex:**

$$ f(x) = x + 3, g(x) = 3x - 1 $$

$$ (\frac{f}{g})(x) = \frac{x + 3}{3x - 1} $$

Note above how we can not factor either the numerator nor the denominator
further. But we do have to state the _Domain_:

$$ (\frac{f}{g})(x) = \frac{x + 3}{3x - 1}, 3x - 1 \neq 0 $$

$$ (\frac{f}{g})(x) = \frac{x + 3}{3x - 1}, 3x \neq 1 $$

**Solution**:

$$ (\frac{f}{g})(x) = \frac{x + 3}{3x - 1}, x \neq \frac{1}{3} $$

---

**Composite Functions**

But _Composite Functions_ are more than just these simple arithmetic operations
with two or more functions. _Composite Functions_ are essentially putting one
function _inside_ another function.

**Composite Function Notation:**

$$ f \circ $$

Do _NOT_ mistake this for "multiply".

What $\circ$ means is "of", meaning it is a _"composition of"_.

$$ (f \circ g)(x) $$

The above can be stated as "$f$ of $g$ of $x$". This also can be read as:

$$ (f \circ g)(x) = f(g(x)) $$

The above is still read the same way, "$f$ of $g$ of $x$".

What this essentially means, is that _"For everywhere you see $x$, in $f(x)$,
you insert the entire function $g(x)$."_

---

**Ex:**

$$ f(x) = x^2, g(x) = 2x + 1 $$

Given these definitions, let's first find _"$f$ of $g$ of $x$"_:

$$ (f \circ g)(x) $$

$$ (f \circ g)(x) = f(g(x)) $$

$$ (f \circ g)(x) = f(g(x)) = f(2x + 1) $$

$$ (f \circ g)(x) = f(g(x)) = f(2x + 1) = (2x + 1)^2 $$

$$ (f \circ g)(x) = (2x + 1)^2 $$

Let's now find _"$g$ of $f$ of $x$"_:

$$ (g \circ f)(x) $$

$$ (g \circ f)(x) = g(f(x)) $$

$$ (g \circ f)(x) = g(f(x)) = g(x^2) $$

$$ (g \circ f)(x) = g(f(x)) = 2(x^2) + 1 $$

$$ (g \circ f)(x) = g(f(x)) = 2x^2 + 1 $$

$$ (g \circ f)(x) = 2x^2 + 1 $$

Note here how $(f \circ g)(x)$ and $(g \circ f)(x) $ do _NOT_ produce the same
output.

Also note that eventually, problem statements will ask you to evaluate specific
values plugged in for $x$ like:

$$ (f \circ g)(3) $$

Or:

$$ (g \circ f)(3) $$

Do _NOT_ attempt to evaluate these expressions first, instead evaluate the
_Composite Function_ first, plugging in for $f$ and $g$ before finding the
solutions to these functions where $x$ is defined.

Let's now evaluate these:

$$ (f \circ g)(3) $$

Since we've evaluated this _Composite Function_ aleady, we simply plug in $3$
for $x$:

$$ (f \circ g)(x) = (2x + 1)^2 $$

$$ (f \circ g)(3) = (2(3) + 1)^2 $$

$$ (f \circ g)(3) = (6 + 1)^2 $$

$$ (f \circ g)(3) = (7)^2 $$

$$ (f \circ g)(3) = 49 $$

And now the other one:

$$ (g \circ f)(3) $$

$$ (g \circ f)(x) = 2x^2 + 1 $$

$$ (g \circ f)(3) = 2(3)^2 + 1 $$

$$ (g \circ f)(3) = 2(9) + 1 $$

$$ (g \circ f)(3) = 18 + 1 $$

$$ (g \circ f)(3) = 19 $$

---

**Practice:**

$$ f(x) = x^2 + 1, g(x) = 3x - 5 $$

$$ (f \circ g)(x) = f(g(x)) $$

$$ (f \circ g)(x) = f(g(x)) = f(3x - 5) $$

$$ (f \circ g)(x) = f(g(x)) = f(3x - 5) = (3x - 5)^2 + 1 $$

$$ (f \circ g)(x) = (3x - 5)^2 + 1 $$

$$ (f \circ g)(4) =  $$

$$ (f \circ g)(4) = (3(4) - 5)^2 + 1 $$

$$ (f \circ g)(4) = (12 - 5)^2 + 1 $$

$$ (f \circ g)(4) = (7)^2 + 1 $$

$$ (f \circ g)(4) = 49 + 1 $$

**Solution:**

$$ (f \circ g)(4) = 50 $$

---

**Practice:**

$$ f(x) = x^2 + 1, g(x) = 3x - 5 $$

$$ (g \circ f)(x) = $$

$$ (g \circ f)(x) = g(f(x)) $$

$$ (g \circ f)(x) = g(x^2 + 1) $$

$$ (g \circ f)(x) = g(x^2 + 1) = 3(x^2 + 1) - 5 $$

$$ (g \circ f)(x) = g(x^2 + 1) = 3x^2 + 3 - 5 $$

$$ (g \circ f)(x) = g(x^2 + 1) = 3x^2 - 2 $$

$$ (g \circ f)(x) = 3x^2 - 2 $$

$$ (g \circ f)(4) =  $$

$$ (g \circ f)(4) = 3(4)^2 - 2 $$

$$ (g \circ f)(4) = 3(16) - 2 $$

$$ (g \circ f)(4) = 48 - 2 $$

**Solution:**

$$ (g \circ f)(4) = 46 $$

---

**Practice:**

$$ f(x) = x^2 + 5, g(x) = \sqrt{x} $$

$$ (f \circ g)(x) = $$

$$ (f \circ g)(x) = f(g(x)) $$

$$ (f \circ g)(x) = f(g(x)) = f(\sqrt{x})$$

$$ (f \circ g)(x) = f(g(x)) = (\sqrt{x})^2 + 5 $$

$$ (f \circ g)(x) = f(g(x)) = x + 5 $$

**Solution:**

$$ (f \circ g)(x) = x + 5 $$

---

**Practice:**

$$ f(x) = x^2 + 5, g(x) = \sqrt{x} $$

$$ (g \circ f)(x) = $$

$$ (g \circ f)(x) = g(f(x)) $$

$$ (g \circ f)(x) = g(f(x)) = g(x^2 + 5) $$

$$ (g \circ f)(x) = g(f(x)) = \sqrt{x^2 + 5} $$

**Solution:**

$$ (g \circ f)(x) = \sqrt{x^2 + 5} $$

---

**Practice:**

$$ f(x) = |x - 4|, g(x) = 3x - 4 $$

$$ (f \circ g)(x) = $$

$$ (f \circ g)(x) = f(g(x)) $$

$$ (f \circ g)(x) = f(g(x)) = f(3x - 4) $$

$$ (f \circ g)(x) = f(g(x)) = f(3x - 4) = |(3x - 4) - 4| $$

$$ (f \circ g)(x) = f(g(x)) = f(3x - 4) = |3x - 4 - 4| $$

$$ (f \circ g)(x) = f(g(x)) = f(3x - 4) = |3x - 8| $$

**Solution:**

$$ (f \circ g)(x) = |3x - 8| $$

---

**Practice:**

$$ f(x) = |x - 4|, g(x) = 3x - 4 $$

$$ (g \circ f)(x) = $$

$$ (g \circ f)(x) = g(f(x)) $$

$$ (g \circ f)(x) = g(f(x)) = g(|x - 4|) $$

$$ (g \circ f)(x) = g(f(x)) = 3(|x - 4|) - 4 $$

**Solution:**

$$ (g \circ f)(x) = 3|x - 4| - 4 $$
