# 12.5: Exploring the Properties of Logarithms

**Note:** Thinking about the Properties of Logarithms as akin to Exponent Rules
can help us understand them.

**Properties Of Logarithms:**

---

_1. Product Property_

$$ log_{b}x\times y =  $$

Let's consider a corresponding Exponent Rule:

$$ x^m \times x^n = x^{m + n} $$

Similarly, we can split up our original logarithm statement as such:

$$ log_{b}x\times y = log_{b}x + log_{b}y $$

Note above that in order fot this property to apply, the split up logarithms
must have the same _Base_, $b$.

**Ex:**

$$ log_{2}7 + log_{2}5 = log_{2}7 \times 5 = log_{2}35 $$

**Ex:**

$$ log_{6}\frac{1}{3} + log_{6}15 = log_{6}\frac{1}{3} \times 15 = log_{6}\frac{15}{3} = log_{6}5 $$

**Ex:**

$$ log_{3}x + log_{3}(x - 9) = log_{3}x \times (x - 9) = log_{3}x(x-9) = log_{3}(x^2-9x) $$

---

**Note:**

A Common mistake made when evaluating logarithms with the _Product Property_:

$$ log_{3}(x + 2) \neq log_{3}x + log_{3}2 $$

---

_2. Quotient Property_

$$ log_{b}\frac{x}{y} $$

Consider our _Exponent Rule_:

$$ \frac{x^m}{x^n} = x^{m - n} $$

Similarly:

$$ log_{b}\frac{x}{y} = log_{b}x - log_{b}y $$

**Ex:**

$$ log_{7}40 - log_{7}8 = log_{7}\frac{40}{8} = log_{7}5 $$

**Ex:**

$$ log_{9}x - log_{9}5 = log_{9}\frac{x}{5} $$

**Ex:**

$$ log_{3}(x^3 + 4) - log_{3}(x^2 + 2) = log_{3}\frac{x^3 + 4}{x^2 + 2}$$

---

**Note:**

Some common mistakes with the _Product Property_ and the _Quotient Property_:

1.

$$ log_{5}x \times log_{5}3 \neq log_{5}3x $$

$$ log_{5}x \times log_{5}3 \neq log_{5}x + log_{5}3 $$

2.

$$ \frac{log_{7}y}{log_{7}3} \neq log_{7}\frac{y}{3} $$

$$ \frac{log_{7}y}{log_{7}3} \neq log_{7}y - log_{7}3 $$

---

**Practice:**

$$ log_{2}\frac{1}{6} + log_{2}18 $$

$$ log_{2}\frac{1}{6} + log_{2}18 = log_{2}(\frac{1}{6} \times 18) $$

$$ log_{2}(\frac{18}{6}) $$

$$ log_{2}(3) $$

---

**Practice:**

$$ log_{6}x - log_{6}3 $$

$$ log_{6}x - log_{6}3 = log_{6}\frac{x}{3} $$

$$  log_{6}\frac{x}{3} $$

---

**Practice:**

$$ log_{5}(x - 1) + log_{5}(x + 1) $$

$$ log_{5}((x - 1)(x + 1)) $$

$$ log_{5}(x^2 - 1) $$

---

**Practice:**

$$ log_{4}(x^2 + 1) - log_{4}(x^2 + 3)$$

$$ log_{4}\frac{x^2 + 1}{x^2 + 3} $$

---

**Practice:**

$$ \frac{log_{4}x}{log_{4}5} $$

$$ \text{NO FURTHER SIMPLIFIED FORM} $$

---

**Practice:**

$$ log_{3}(x - 1) \times log_{3}(x + 1) $$

$$ \text{NO FURTHER SIMPLIFIED FORM} $$

---

_3. Power Property_

$$ log_{b}x^r $$

Recall the _Exponent Rule_:

$$ (x^m)^n = x^{m \times n} = x^{mn} $$

Similary:

$$ log_{b}x^r = r \times log_{b}x $$

**Ex:**

$$ log_{3}x^5 = 5log_{b}x $$

**Ex:**

$$ log_{7}\sqrt[3]{4} = log_{7}4^{\frac{1}{3}} = \frac{1}{3}log_{7}4 $$

This can also be expressed as:

$$ \frac{log_{7}4}{3} $$

---

**Practice:**

$$ log_{6}x^8 $$

$$ 8log_{6} $$

---

**Practice:**

$$ log_{2}\sqrt[4]{x} $$

$$ log_{2}x^{\frac{1}{4}} $$

$$ \frac{1}{4}log_{2}x $$

$$ \frac{log_{2}x}{4} $$

---

**Combining Logarithms**

**Ex:**

$$ 3log_{4}2 + 2log_{4}5 $$

First let's take care of any numbers that might be exponents. In other words,
_Numbers In Front of Our Logarithms_. In this case, that would be $3$ and $2$.
Thusly, we can rewrite our initial problem statement as such:

$$ log_{4}2^3 + log_{4}5^2 $$

Now can use the _Product Property_ to further simplify:

$$ log_{4}(2^3 \times 5^2) $$

$$ log_{4}(8 \times 25) $$

$$ log_{4}200 $$

---

**Ex:**

$$ 5log_{2}(2x - 1) - log_{2}x $$

$$ log_{2}(2x - 1)^5 - log_{2}x $$

$$ log_{2}\frac{(2x - 1)^5}{x} $$

---

**Ex:**

$$ log_{11}8 + log_{11}3 - log_{11}2 $$

$$ log_{11}(8 \times 3) - log_{11}2 $$

$$ log_{11}24 - log_{11}2 $$

$$ log_{11}\frac{24}{2} $$

$$ log_{11}12 $$

---

**Ex:**

$$ 2log_{5}4 + 5log_{5}2 $$

$$ log_{5}4^2 + log_{5}2^5 $$

$$ log_{5}(4^2 \times 2^5) $$

$$ log_{5}(16 \times 32) $$

$$ log_{5}(512) $$

---

**Ex:**

$$ \frac{1}{2}log_{8}x - log_{8}(x + 3) $$

$$ log_{8}x^{\frac{1}{2}} - log_{8}(x + 3) $$

$$ log_{8}(\frac{x^{\frac{1}{2}}}{x+3}) $$

$$ log_{8}\frac{\sqrt{x}}{x+3} $$

---

**Expand**

**Ex:**

$$ log_{7}(\frac{6 \times 2}{5}) $$

$$ log_{7}(6 \times 2) - log_{7}5 $$

$$ log_{7}6 + log_{7}2 - log_{7}5 $$

**Ex:**

$$ log_{3}\frac{x^4}{y^3} $$

$$ log_{3}x^4 - log_{3}y^3 $$

$$ 4log_{3}x - 3log_{3}y $$

---

**Practice:**

$$ log_{5}\frac{4 \times 3}{7} $$

$$ log_{5}(4 \times 3) - log_{5}7 $$

$$ log_{5}4 + log_{5}3 - log_{5}7 $$

---

**Practice:**

$$ log_{4}\frac{a^2}{b^{\frac{1}{4}}} $$

$$ log_{4}a^2 - log_{4}b^{\frac{1}{4}} $$

$$ 2log_{4}a - \frac{1}{4}log_{4}b $$

---

Let's suppose you only know two _Logarithms_ in the world:

$$ log_{b}4 = 0.87, log_{b}7 = 121 $$

---

$$ log_{b}28 = log_{b}(4 \times 7) = log_{b}4 + log_{b}7 $$

$$ log_{b}28 = 0.87 + 121 $$

$$ log_{b}28 = 121.87 $$

---

Let's continue to substitute in:

$$ log_{b}49 = log_{b}7^2 = 2log_{b}7 $$

$$ log_{b}49 = 2(121) $$

$$ log_{b}49 = 242 $$

---

And again:

$$ log_{b}\sqrt[3]{4} = log_{b}4^{\frac{1}{3}} = \frac{1}{3}log_{b}4 $$

$$ log_{b}\sqrt[3]{4} = \frac{1}{3}(0.87)$$

$$ log_{b}\sqrt[3]{4} = 0.29 $$
