# 7.5: Solving Rational Equations (Equations with Rational Expressions)

**Steps:**

1. Find LCD.
   - Might factor 1st.

2. Multiply <em>every term</em> by the LCD.
   - **NOTE:**

   <b>NOT</b>

   $$ \frac{LCD}{LCD} $$

   _This will eliminate denominators_

---

**Ex:**

$$ \frac{x}{4} + \frac{4}{5} = \frac{1}{20} $$

$$ LCD = 20 $$

$$ \frac{20}{1}\times(\frac{x}{4} + \frac{4}{5}) = \frac{1}{20}\times(\frac{20}{1}) $$

$$ (\frac{5}{1}\times\frac{x}{1}) + (\frac{4}{1}\times\frac{4}{1}) = 1 $$

$$ 5x + 16 = 1 $$

$$ 5x = 15 $$

<ins>Answer:</ins>

$$ x = 3 $$

---

**Ex:**

$$ \frac{x+2}{3} - \frac{x-1}{5} = 15 $$

$$ LCD = 15 $$

$$ \frac{15}{1}\times\frac{x+2}{3} - \frac{15}{1}\times\frac{x-1}{5} = \frac{15}{1}\times\frac{15}{1} $$

$$ \frac{5}{1}\times\frac{x+2}{1} - \frac{3}{1}\times\frac{x-1}{1} = \frac{225}{1} $$

$$ 5(x+2) - (3(x-1)) = 225 $$

$$ 5x + 10 - (3x - 3)  = 225 $$

$$ 5x + 10 - 3x + 3 = 225 $$

$$ 2x + 13 = 225 $$

$$ 2x = 212 $$

<ins>Answer:</ins>

$$ x = 106 $$

---

**Ex:**

$$ \frac{x+4}{4} - \frac{x-3}{3} = \frac{1}{12} $$

$$ LCD = 12 $$

$$ \frac{12}{1}\times\frac{x+4}{4} - \frac{12}{1}\times\frac{x-3}{3} = \frac{1}{12}\times\frac{12}{1} $$

$$ \frac{3}{1}\times\frac{x+4}{1} - \frac{4}{1}\times\frac{x-3}{1} = 1 $$

$$ 3(x+4) - (4(x-3)) = 1 $$

$$ 3x + 12 - (4x - 12) = 1 $$

$$ 3x + 12 - 4x + 12 = 1 $$

$$ -x + 24 = 1 $$

$$ -x = -23 $$

<ins>Answer:</ins>

$$ x = 23 $$

---

**Ex:**

$$ 2 + \frac{6}{x} = x + 7 $$

$$ \frac{2}{1} + \frac{6}{x} = \frac{x}{1} + \frac{7}{1} $$

$$ LCD = x $$

$$ \frac{x}{1}\times\frac{2}{1} + \frac{x}{1}\times\frac{6}{x} = \frac{x}{1}\times\frac{x}{1} + \frac{x}{1}\times\frac{7}{1} $$

$$ 2x + 6 = x^2 + 7x $$

$$ 2x + 6 - (x^2 + 7x) = 0 $$

$$ 2x + 6 - x^2 - 7x = 0 $$

$$ -x^2 - 5x + 6 = 0 $$

$$ x^2 + 5x - 6 = 0 $$

$$ (x + 6)(x - 1) = 0 $$

$$ x + 6 = 0 $$

$$ x - 1 = 0 $$

<ins>Answer:</ins>

$$ x = -6 $$

$$ x = 1 $$

---

**Ex:**

$$ \frac{7x}{x^2+2x-15} - \frac{4}{x-3} = -\frac{2}{x+5} $$

$$ \frac{7x}{(x+5)(x-3)} - \frac{4}{x-3} = -\frac{2}{x+5} $$

$$ LCD = (x+5)(x-3) $$

$$ \frac{(x+5)(x-3)}{1}\times\frac{7x}{(x+5)(x-3)} - \frac{(x+5)(x-3)}{1}\times\frac{4}{x-3} = -\frac{2}{x+5}\times\frac{(x+5)(x-3)}{1}  $$

$$ \frac{1}{1}\times\frac{7x}{1} - \frac{x+5}{1}\times\frac{4}{1} = -\frac{2}{1}\times\frac{x-3}{1} $$

$$ 7x - (4(x+5)) = -2(x-3) $$

$$ 7x - (4x+20) = -2(x-3) $$

$$ 7x - 4x - 20 = -2x+6 $$

$$ 3x - 20 = 6 - 2x$$

$$ 3x - 20 - (6 - 2x) = 0 $$

$$ 3x - 20 - 6 + 2x = 0 $$

$$ 5x - 26 = 0 $$

$$ 5x = -26 $$

<ins>Answer:</ins>

$$ x = -\frac{26}{5} $$

---

**Ex:**

$$ \frac{5x}{x-1} = \frac{5}{x-1} + 3 $$

$$ \frac{5x}{x-1} = \frac{5}{x-1} + \frac{3}{1} $$

$$ LCD = x - 1 $$

$$ \frac{x-1}{1}\times\frac{5x}{x-1} = \frac{x-1}{1}\times\frac{5}{x-1} + \frac{x-1}{1}\times\frac{3}{1} $$

$$ 5x = 5 + 3(x-1) $$

$$ 5x = 5 + 3x - 3 $$

$$ 5x = 3x + 2 $$

$$ 5x - (3x + 2) = 0 $$

$$ 5x - 3x - 2 = 0 $$

$$ 2x - 2 = 0 $$

$$ 2x = 2 $$

<ins>FALSE SOLUTION:</ins>

$$ \cancel{x = 1} $$

NOTE: False because if we plug in $1$ to the above, we get a division by zero
error.

---

**Ex:**

$$ 8 + \frac{7}{x} = x + 2 $$

$$ \frac{8}{1} + \frac{7}{x} = \frac{x}{1} + \frac{2}{1} $$

$$ LCD = x $$

$$ \frac{x}{1}\times\frac{8}{1} + \frac{x}{1}\times\frac{7}{x} = \frac{x}{1}\times\frac{x}{1} + \frac{x}{1}\times\frac{2}{1} $$

$$ 8x + 7 = x^2 + 2x $$

$$ 0 = x^2 + 2x - (8x + 7) $$

$$ x^2 + 2x - (8x + 7) = 0 $$

$$ x^2 + 2x - 8x - 7 = 0 $$

$$ x^2 - 6x - 7 = 0 $$

$$ (x - 7)(x + 1) = 0 $$

$$ x - 7 = 0 $$

$$ x + 1 = 0 $$

<ins>Answer:</ins>

$$ x = 7 $$

$$ x = -1 $$

---

**Ex:**

$$ \frac{6x}{x^2-5x-14} - \frac{3}{x+2} = \frac{1}{x-7} $$

$$ \frac{6x}{(x-7)(x+2)} - \frac{3}{x+2} = \frac{1}{x-7} $$

$$ LCD = (x-7)(x+2) $$

$$ \frac{(x-7)(x+2)}{1}\times\frac{6x}{(x-7)(x+2)} - \frac{(x-7)(x+2)}{1}\times\frac{3}{x+2} = \frac{(x-7)(x+2)}{1}\times\frac{1}{x-7} $$

$$ 6x - (3(x-7)) = x + 2 $$

$$ 6x - (3x - 21) = x + 2 $$

$$ 6x - 3x + 21 = x + 2 $$

$$ 3x + 21 = x + 2 $$

$$ 3x + 21 - (x + 2) = 0 $$

$$ 3x + 21 - x - 2 = 0 $$

$$ 2x + 19 = 0 $$

$$ 2x = -19 $$

<ins>Answer:</ins>

$$ x = -\frac{19}{2} $$

---

**Ex:**

$$ x - \frac{6}{x+3} = \frac{2x}{x+3} + 2  $$

$$ \frac{x}{1} - \frac{6}{x+3} = \frac{2x}{x+3} + \frac{2}{1}  $$

$$ LCD = x+3 $$

$$ \frac{x+3}{1}\times\frac{x}{1} - \frac{x+3}{1}\times\frac{6}{x+3} = \frac{x+3}{1}\times\frac{2x}{x+3} + \frac{x+3}{1}\times\frac{2}{1} $$

$$ x(x+3) - 6 = 2x + 2(x+3) $$

$$ x^2 + 3x - 6 = 2x + 2x + 6 $$

$$ x^2 + 3x - 6 = 4x + 6 $$

$$ x^2 + 3x - 6 - (4x + 6) = 0 $$

$$ x^2 + 3x - 6 - 4x - 6 = 0 $$

$$ x^2 - x - 12 = 0 $$

$$ (x + 3)(x - 4) = 0 $$

$$ x + 3 = 0 $$

$$ x - 4 = 0 $$

<ins>Answer:</ins>

$$ \cancel{x = -3} $$

$$ x = 4 $$
