# 11.1 Solving Quadratic Equations By Completing the Square

_Quadratic Equation_: Any equation where the largest power of some variable is
$2$.

This is also referred to as a _$2$<sup>nd</sup> degree equation_.

$$ ax^2 +bx +c = 0 $$

**Ex:**

$$ x^2 = 9 $$

Note that there are two ways of solving this equation:

Method 1: Move all to 1 side and then factor:

$$ x^2 - 9 = 0 $$

$$ (x + 3)(x - 3)= 0 $$

$$ x + 3 = 0, x - 3 = 0 $$

$$ x = -3, x = 3 $$

Method 2: Take the square root of both sides to find the answer:

$$ x^2 = 9 $$

$$ \sqrt{x^2} = \sqrt{9} $$

$$ x = 3 $$

But notice that we only get _one_ solution here, this is a _problem_. We can fix
this by noting this using the _Plus Or Minus_ symbole:

$$ x^2 = 9 $$

$$ \sqrt{x^2} = \pm\sqrt{9} $$

$$ x = \pm3 $$

Which is short hand for:

$$ x = -3, x = 3 $$

Note that whenever you take the square root to solve for the value of a variable
in an equation, you _Must include the Plus Or Minus Notation_. This means that
_if you put the square root on your solution, you Must include the Plus Or Minus
symbol, this gives two solution_.

---

**Ex:**

$$ x^2 = 20 $$

$$ x^2 = (5 \times 4) $$

$$ \sqrt{x^2} = \pm\sqrt{(5 \times 4)} $$

$$ x = \pm2\sqrt{5} $$

Note where the $\pm$ symbol should go. For example, this expression notes that
the solution is _not equal_ to $2\pm\sqrt{5}$:

$$ x \neq 2\pm\sqrt{5} $$

---

**Ex:**

$$ x^2 = 18 $$

$$ x^2 = (9 \times 3) $$

$$ \sqrt{x^2} = \pm\sqrt{(9 \times 3)} $$

$$ x = \pm3\sqrt{3} $$

$$ x = 3\sqrt{3}, -3\sqrt{3} $$

---

**Ex:**

$$ 5x^2 - 55 = 0 $$

$$ 5x^2 = 55 $$

$$ \frac{5x^2}{5} = \frac{55}{5} $$

$$ x^2 = 11 $$

$$ \sqrt{x^2} = \pm\sqrt{11} $$

$$ x = \pm\sqrt{11} $$

$$ x= \sqrt{11}, -\sqrt{11} $$

---

**Practice:**

$$ 3x^2 - 30 = 0 $$

$$ 3x^2 = 30 $$

$$ \frac{3x^2}{3} = \frac{30}{3} $$

$$ x^2 = 10 $$

$$ \sqrt{x^2} = \pm\sqrt{10} $$

$$ x = \pm\sqrt{10} $$

$$ x = \sqrt{10}, -\sqrt{10} $$

---

**Practice:**

$$ (x + 2)^2 = 18 $$

$$ \sqrt{(x + 2)^2} = \pm\sqrt{18} $$

$$ x + 2 = \pm\sqrt{9 \times 2} $$

$$ x + 2 = \pm3\sqrt{2} $$

$$ x = -2 \pm3\sqrt{2} $$

$$ x = -2 + 3\sqrt{2}, -2 - 3\sqrt{2} $$

---

**Ex:**

$$ (x + 3)^2 = 20 $$

$$ \sqrt{(x + 3)^2} = \pm\sqrt{20} $$

$$ x + 3 = \pm\sqrt{20} $$

$$ x + 3 = \pm\sqrt{5 \times 4} $$

$$ x + 3 = \pm2\sqrt{5} $$

$$ x = -3 \pm2\sqrt{5} $$

$$ x = -3 + 2\sqrt{5}, -3 - 2\sqrt{5} $$

---

**Ex:**

$$ (3x - 1)^2 = -4 $$

$$ \sqrt{(3x - 1)^2} = \pm\sqrt{-4} $$

$$ 3x - 1 = \pm\sqrt{-4} $$

$$ 3x - 1 = \pm\sqrt{-1 \times 4} $$

$$ 3x - 1 = \pm(\sqrt{-1} \times \sqrt{4}) $$

$$ 3x - 1 = \pm(i \times 2) $$

$$ 3x - 1 = \pm2i $$

$$ 3x = 1 \pm 2i $$

$$ \frac{3x}{3} = \frac{1 \pm 2i}{3} $$

$$ x = \pm(\frac{1 \pm 2i}{3}) $$

$$ x = \frac{1 + 2i}{3}, \frac{1 - 2i}{3} $$

$$ x = \frac{1}{3} + \frac{2}{3}i, \frac{1}{3} - \frac{2}{3}i $$

---

**Ex:**

$$ (5x - 2)^2 + 2 = -7 $$

$$ (5x - 2)^2 = -9 $$

$$ \sqrt{(5x - 2)^2} = \pm\sqrt{-9} $$

$$ 5x - 2 = \pm\sqrt{-9} $$

$$ 5x - 2 = \pm\sqrt{-1 \times 9} $$

$$ 5x - 2 = \pm\sqrt{-1} \times \sqrt{9} $$

$$ 5x - 2 = \pm(i \times 3) $$

$$ 5x - 2 = \pm3i $$

$$ 5x = 2 \pm 3i $$

$$ \frac{5x}{5} = \frac{2 \pm 3i}{5} $$

$$ x = \frac{2 \pm 3i}{5} $$

$$ x = \frac{2 + 3i}{5}, \frac{2 - 3i}{5} $$

$$ x = \frac{2}{5} + \frac{3}{5}i, \frac{2}{5} - \frac{3}{5}i $$

---

**Ex:**

$$ x^2 + 8x + 16 = 0 $$

---

**Ex:**

Note the pattern with each of these, take the _second term_, divide it by $2$,
then _square_ the result, it will always give you the _third term_, indicating
what will be the result $(x + \text{ result})^2$ or
$(x + \frac{\text{ second term}}{2})^2$.

$$ x^2 + 8x + 16 = (x + 4)^2 $$

$$ x^2 - 6x + 9 = (x - 3)^2 $$

$$ x^2 + 3x + \frac{9}{4} = (x + \frac{3}{2})^2 $$

These are examples of a _Perfect Square Trinomial_. Again, this is indicated if
the _third term_ is _half the second term squared_, then it is a _Perfect Square
Trinomial_.

But the above are demonstrations of equivalency, usually you will see an
equation like this:

$$ x^2 + 8x = 1 $$

Even when we get all our terms to one side of the equation, this does _NOT_
fulfill our definition of a _Perfect Square Trinomial_.

$$ x^2 + 8x - 1 = 0 $$

Note that $-1$ is _NOT_ _half the second term, $8x$ squared_, and therefore is
_NOT_ a _Perfect Sqaure Trinomial_.

The solution is to "force" our left hand side of the initial equation to fit the
requirements for a _Perfect Square Trinomial_.

We can find out what our _third term_ should be by taking the _second term_,
_halfing it_, and then _squaring the result_.

$$ (\frac{8}{2})^2 = 16 $$

We can then _add this to both sides of our equation like so:

$$ x^2 + 8x = 1 $$

$$ x^2 + 8x + 16 = 1 + 16 $$

$$ x^2 + 8x + 16 = 17 $$

$$ (x + 4)^2 = 17 $$

$$ \sqrt{(x + 4)^2} = \pm\sqrt{17} $$

$$ x + 4 = \pm\sqrt{17} $$

$$ x = -4 \pm\sqrt{17} $$

$$ x = -4 + \sqrt{17}, -4 - \sqrt{17} $$

---

We're now going to slow down, and go through each of the steps we did to solve
the previous problem. When you are asked to solve the equation by _completing
the square_, do the following:

**Steps:**

1. Set up the equation so that the $x$-terms are on one side of the equation and
   the constant is on the other.

$$ x^2 + 8x = 1 $$

2. Make sure the coefficient of the $x^2$ term is $1$, otherwise you will have
   to divide to ensure the coefficient of the $x^2$ term is $1$.

$$ x^2 + 8x = 1 $$

3. Add the _square_ of _half_ the coefficient of the $x$ term to both sides of
   the equation.

$$ x^2 + 8x = 1 $$

$$ (\frac{8}{2})^2 = 16 $$

$$ x^2 + 8x + 16 = 1 + 16 $$

$$ x^2 + 8x + 16 = 17 $$

Once we are at this step, we can start to factor and solving this.

4. Factor (_Pefect Square Trinomial_).

Because we have "forced" the left hand side of our equation to be a _Perfect
Square Trinomial_, we can easily determine what term needs to be squared on the
left hand side:

$$ (x + 4)^2 = 17 $$

$$ \sqrt{(x + 4)^2} = \pm\sqrt{17} $$

$$ x + 4 = \pm\sqrt{17} $$

$$ x = -4 \pm\sqrt{17} $$

$$ x = -4 + \sqrt{17}, -4 - \sqrt{17} $$

---

**Ex:**

$$ y^2 + 4y - 3 = 0 $$

$$ y^2 + 4y = 3 $$

$$ (\frac{4}{2})^2 = 4 $$

$$ y^2 + 4y + 4 = 3 + 4 $$

$$ y^2 + 4y + 4 = 7 $$

$$ (y + 2)^2 = 7 $$

$$ \sqrt{(y + 2)^2} = \pm\sqrt{7} $$

$$ y + 2 = \pm\sqrt{7} $$

$$ y = -2 \pm\sqrt{7} $$

$$ y = -2 + \sqrt{7}, -2 - \sqrt{7} $$

---

**Ex:**

$$ x^2 - 5x + 2 = 0 $$

$$ x^2 - 5x = -2 $$

$$ (\frac{-5}{2})^2 = \frac{25}{4} $$

$$ x^2 - 5x + \frac{25}{4} = -2 + \frac{25}{4} $$

$$ x^2 - 5x + \frac{25}{4} = -\frac{8}{4} + \frac{25}{4} $$

The left hand side is hard to see, but you can easily figure it out since this
is a _Perfect Square Trinomial_, simply take the _middle term_ divided by $2$,
and that is what is our second term within the squared left hand side:

$$ (x - \frac{5}{2})^2= \frac{17}{4} $$

$$ \sqrt{(x - \frac{5}{2})^2} = \pm\sqrt{\frac{17}{4}} $$

$$ x - \frac{5}{2} = \pm\sqrt{\frac{17}{4}} $$

$$ x = \frac{5}{2} \pm\sqrt{\frac{17}{4}} $$

$$ x = \frac{5}{2} \pm\frac{\sqrt{17}}{2} $$

$$ x = \frac{5 \pm\sqrt{17}}{2} $$

$$ x = \frac{5 + \sqrt{17}}{2}, \frac{5 - \sqrt{17}}{2} $$

---

**Ex:**

Let's handle one with an $x^2$ term coefficent:

$$ 3x^2 - 12x + 1 = 0 $$

$$ 3x^2 - 12x = -1 $$

To get rid of the $3$ $x^2$ coefficient, we'll need to divide _all terms_ by
$3$:

$$ \frac{3x^2}{3} - \frac{12x}{3} = \frac{-1}{3} $$

$$ x^2 - 4x = -\frac{1}{3} $$

$$ (\frac{-4}{2})^2 = 4 $$

$$ x^2 - 4x + 4 = -\frac{1}{3} + 4 $$

$$ (x - 2)^2= -\frac{1}{3} + \frac{12}{3} $$

$$ (x - 2)^2= \frac{11}{3} $$

We leave it here for now, this is just a demonstration of how to deal with the
$x^2$ term coefficient.

---

**Ex:**

$$ y^2 + 4y - 3 = 0 $$

$$ y^2 + 4y = 3 $$

$$ (\frac{4}{2})^2 = 4 $$

$$ y^2 + 4y + 4= 3 + 4 $$

$$ y^2 + 4y + 4= 7 $$

$$ (y + 2)^2 = 7 $$

$$ \sqrt{(y + 2)^2} = \pm\sqrt{7} $$

$$ y + 2 = \pm\sqrt{7} $$

$$ y = -2 \pm\sqrt{7} $$

$$ y = -2 + \sqrt{7}, -2 - \sqrt{7}  $$

---

**Ex:**

$$ x^2 - 5x + 2 = 0 $$

$$ x^2 - 5x = -2 $$

$$ (\frac{-5}{2})^2 = \frac{25}{4} $$

We can skip a step on the left, because we know that _half of our second term_
is the amount we can add (whether positive or negative) to our $x$ term inside
of a _squared term_:

$$ (x - \frac{5}{2})^2 $$

$$ (x - \frac{5}{2})^2 = -2 + \frac{25}{4} $$

$$ (x - \frac{5}{2})^2 = \frac{-8}{4} + \frac{25}{4} $$

$$ (x - \frac{5}{2})^2 = \frac{17}{4} $$

$$ \sqrt{(x - \frac{5}{2})^2} = \pm\sqrt{\frac{17}{4}} $$

$$ x - \frac{5}{2} = \pm\sqrt{\frac{17}{4}} $$

$$ x - \frac{5}{2} = \pm \frac{\sqrt{17}}{2} $$

$$ x = \frac{5}{2} \pm \frac{\sqrt{17}}{2} $$

$$ x = \frac{5 \pm\sqrt{17}}{2} $$

---

**Ex:**

$$ 2x^2 - 5x + 7 = 0 $$

$$ 2x^2 - 5x = -7 $$

$$ \frac{2x^2}{2} - \frac{5}{2} = -\frac{7}{2} $$

$$ x^2 - \frac{5}{2} = -\frac{7}{2} $$

$$ (\frac{-\frac{5}{2}}{2})^2 = (-\frac{5}{2} \times \frac{1}{2})^2 = (-\frac{5}{4})^2 = \frac{25}{16} $$

$$ (x - \frac{5}{4})^2 = -\frac{7}{2} + \frac{25}{16} $$

$$ (x - \frac{5}{4})^2 = -\frac{56}{16} + \frac{25}{16} $$

$$ (x - \frac{5}{4})^2 = -\frac{31}{16} $$

$$ \sqrt{(x - \frac{5}{4})^2} = \pm\sqrt{-\frac{31}{16}} $$

$$ x - \frac{5}{4} = \pm\sqrt{-1(\frac{31}{16})} $$

$$ x - \frac{5}{4} = \pm i\sqrt{\frac{31}{16}} $$

$$ x - \frac{5}{4} = \pm i\frac{\sqrt{31}}{4} $$

$$ x = \frac{5}{4} \pm i\frac{\sqrt{31}}{4} $$

$$ x = \frac{5 \pm i\sqrt{31}}{4} $$

$$ x = \frac{5}{4} \pm \frac{\sqrt{31}}{4}i $$

---

Let's now look at the Quadratic Equation formula to more easily see the exact
process, step by step:

$$ ax^2 + bx + c = 0 $$

$$ ax^2 + bx = -c $$

$$ \frac{ax^2}{a} + \frac{bx}{a} = \frac{-c}{a} $$

$$ x^2 + \frac{b}{a}x = -\frac{c}{a} $$

$$ x^2 + \frac{b}{a}x + (\frac{b}{2a})^2 = -\frac{c}{a} + (\frac{b}{2a})^2 $$

$$ (x + \frac{b}{2a})^2 = \frac{-c}{a} + (\frac{b}{2a})^2 $$

$$ (x + \frac{b}{2a})^2 = \frac{-c}{a} + \frac{b^2}{4a^2} $$

$$ (x + \frac{b}{2a})^2 = \frac{-4ac}{4a^2} + \frac{b^2}{4a^2} $$

$$ (x + \frac{b}{2a})^2 = \frac{b^2 - 4ac}{4a^2} $$

$$ \sqrt{(x + \frac{b}{2a})^2} = \pm\sqrt{\frac{b^2 - 4ac}{4a^2}} $$

$$ x + \frac{b}{2a} = \pm\sqrt{\frac{b^2 - 4ac}{4a^2}} $$

$$ x + \frac{b}{2a} = \pm \frac{\sqrt{b^2 - 4ac}}{2a} $$

$$ x = -\frac{b}{2a} \pm \frac{\sqrt{b^2 - 4ac}}{2a} $$

$$ x = \frac{-b \pm \sqrt{b^2 - 4ac}}{2a} $$

The above is what is known as the
[Quadratic Formula](https://en.wikipedia.org/wiki/Quadratic_formula).
