# 11.3: Solving Equations Using Various Quadratic Methods

**Applications of Quadratic Methods**

**Steps:**

1. If you have $()^2 = c$, take the $\sqrt{}$ with the $\pm$.A

2. Force the format of your equation into $ax^2 + bx + c = 0$ if it is not
   already in the _Quadratic Formula_ format.

3. Try to factor (~10 seconds).

4. If you can't factor quickly, then use the _Quadratic Formula_.

---

**Ex:**

$$ x - \sqrt{x - 1} - 3 = 0 $$

$$ x - 3 = \sqrt{x - 1} $$

$$ (x - 3)^2 = (\sqrt{x - 1})^2 $$

$$ (x - 3)(x - 3) = x - 1 $$

$$ x^2 - 6x + 9 = x - 1 $$

$$ x^2 - 7x + 10 = 0 $$

$$ (x -2)(x - 5) = 0 $$

$$ x - 2 = 0, x - 5 = 0 $$

$$ x = 2, x = 5 $$

Check work:

$$ x - \sqrt{x - 1} - 3 = 0 $$

$$ x = 2 $$

$$ 2 - \sqrt{2 - 1} - 3 = 0 $$

$$ 2 - \sqrt{1} - 3 = 0 $$

$$ 2 - 1 - 3 = 0 $$

$$ 1 - 3 = 0 $$

$$ -2 \neq 0 $$

Check work:

$$ x - \sqrt{x - 1} - 3 = 0 $$

$$ x = 5 $$

$$ 5 - \sqrt{5 - 1} - 3 = 0 $$

$$ 5 - \sqrt{4} - 3 = 0 $$

$$ 5 - 2 - 3 = 0 $$

$$ 3 - 3 = 0 $$

$$ 0 = 0 $$

Therefore our answer is:

$$ x = 5 $$

---

**Ex:**

$$ \frac{2x}{x - 1} - \frac{x + 2}{x} = \frac{5}{x(x - 1)} $$

$$ LCD = x(x - 1) $$

$$ (\frac{x(x - 1)}{1})(\frac{2x}{x - 1}) - (\frac{x(x - 1)}{1})(\frac{x + 2}{x}) = (\frac{5}{x(x - 1)})(\frac{x(x - 1)}{1}) $$

$$ x(2x) - (x - 1)(x + 2) = 5 $$

$$ 2x^2 - (x^2 -x + 2x - 2) = 5 $$

$$ 2x^2 - (x^2 + x - 2) = 5 $$

$$ 2x^2 - x^2 - x + 2 = 5 $$

$$ x^2 - x + 2 = 5 $$

$$ x^2 - x - 3 = 0 $$

$$ a = 1 $$

$$ b = -1 $$

$$ c = -3 $$

$$ x = \frac{-(-1) \pm \sqrt{(-1)^2 - 4(1)(-3)}}{2(1)} $$

$$ x = \frac{1 \pm \sqrt{1 + 12}}{2} $$

$$ x = \frac{1 \pm \sqrt{13}}{2} $$

$$ x = \frac{1 + \sqrt{13}}{2}, \frac{1 - \sqrt{13}}{2} $$

---

**Ex:**

$$ x^4 - 5x^2 - 36 = 0 $$

Not a _Quadratic Formula_, but we can "force" it into one. We can do this by
_Making A Substitution_:

$$ (x^2)^2 - 5(x^2) - 36 = 0 $$

We can then assign $x^2$ to a dummy variable, $y$.

$$ y = x^2 $$

And then rewrite your equation into something more familiar:

$$ y^2 - 5y - 36 = 0 $$

$$ (y - 9)(y + 4) = 0 $$

$$ y - 9 = 0, y + 4 = 0 $$

$$ y = 9, y = -4 $$

$$ x^2 = 9, x^2 = -4 $$

$$ \sqrt{x^2} = \pm\sqrt{9}, \sqrt{x^2} = \pm\sqrt{-4} $$

$$ x = \pm3, x = \pm\sqrt{-1 \times 4} $$

$$ x = \pm3, x = \pm i\sqrt{4} $$

$$ x = \pm3, x = \pm2i $$

$$ x = 3, x = -3, x = 2i, x = -2i $$

---

**Ex:**

$$ x^4 - 7x^2 - 144 = 0 $$

What we're doing with these $x^4$ starting equations, called _Quartic
Equations_, is turn them into _Quadratic Equations_, so that we can easily use
our _Quadratic Formula_ to solve for $x$.

We can start by rewriting $x^4$ as $(x^2)^2$:

$$ (x^2)^2 - 7(x^2) - 144 = 0 $$

We can then substitute in a dummy variable $y$ for $x^2$ as long as we don't
forget to substitute $x^2$ back in for $y$ at the end of solving our problem.

$$ y = x^2 $$

$$ y^2 - 7y - 144 = 0 $$

$$ (y - 16)(y + 9) = 0 $$

$$ y - 16 = 0, y + 9 = 0 $$

$$ y = 16, y = -9 $$

$$ x^2 = 16, x^2 = -9 $$

$$ \sqrt{x^2} = \pm\sqrt{16}, \sqrt{x^2} = \pm\sqrt{-9} $$

$$ x = \pm4, x = \pm\sqrt{-1 \times 9} $$

$$ x = \pm4, x = \pm i\sqrt{9} $$

$$ x = \pm4, x = \pm3i $$

$$ x = 4, x = -4, x = 3i, x = -3i $$

---

$$ (x + 4)^2 - (x + 4) - 6 = 0 $$

$$ y = x + 4 $$

$$ y^2 - y - 6 = 0  $$

$$ (y - 3)(y + 2) = 0 $$

$$ y - 3, y + 2 = 0 $$

$$ y = 3, y = -2 $$

$$ x + 4 = 3, x + 4 = -2 $$

$$ x = -1, x = -6 $$

---

$$ x^{\frac{2}{3}} - 7x^{\frac{1}{3}} + 10 = 0 $$

Note here that $x^{\frac{2}{3}}$ is equivalent to $(x^{\frac{1}{3}})^2$

$$ y = x^{\frac{1}{3}} $$

$$ y^2 - 7y + 10 = 0 $$

$$ (y - 5)(y - 2)= 0 $$

$$ y - 5 = 0, y - 2 = 0 $$

$$ y = 5, y = 2 $$

$$ x^{\frac{1}{3}} = 5, x^{\frac{1}{3}} = 2 $$

$$ (x^{\frac{1}{3}})^3 = 5^3, (x^{\frac{1}{3}})^3 = 2^3 $$

$$ x = 125, x = 8 $$

---

**Ex:**

$$ x^{\frac{2}{3}} - 5x^{\frac{1}{3}} + 4 = 0 $$

$$ y = x^{\frac{1}{3}} $$

$$ y^2 - 5y + 4 = 0 $$

$$ (y - 4)(y - 1) = 0 $$

$$ y - 4 = 0, y - 1 = 0 $$

$$ y = 4, y = 1 $$

$$ x^{\frac{1}{3}} = 4, x^{\frac{1}{3}} = 1 $$

$$ (x^{\frac{1}{3}})^3 = 4^3, (x^{\frac{1}{3}})^3 = 1^3 $$

$$ x = 64, x = 1 $$

---

<ins>Work Time</ins>: Karen and Doug can clean a house together in $5$ hours
alone. Karen can clean it in $1$ hour faster than Doug. How fast can each person
clean the house alone?

|          | Total Time | Per Hour |
| -------- | ---------- | -------- |
| Doug     | x          | 1/x      |
| Karen    | x - 1      | 1/(x-1)  |
| Together | 5          | 1/5      |

$$ \text{Doug Per Hour} + \text{Karen Per Hour} = \text{Together Per Hour} $$

$$ D + K = T $$

$$ \frac{1}{x} + \frac{1}{x - 1} = \frac{1}{5} $$

$$ LCD = 5(x)(x-1) $$

$$ (\frac{5(x)(x-1)}{1})(\frac{1}{x}) + (\frac{5(x)(x-1)}{1})(\frac{1}{x - 1}) = (\frac{5(x)(x-1)}{1})(\frac{1}{5}) $$

$$ 5(x - 1) + 5x = x(x - 1) $$

$$ 5x - 5 + 5x = x^2 - x $$

$$ 10x - 5 = x^2 - x $$

$$ 0 = x^2 - x - 10x + 5 $$

$$ 0 = x^2 - 11x + 5 $$

Use _Quadratic Formula_:

$$ a = 1 $$

$$ b = -11 $$

$$ c = 5 $$

$$ x = \frac{-(-11) \pm \sqrt{(-11)^2 - 4(1)(5)}}{2(1)} $$

$$ x = \frac{11 \pm \sqrt{121 - 20}}{2} $$

$$ x = \frac{11 \pm \sqrt{101}}{2} $$

$$ x = \frac{11 + \sqrt{101}}{2}, x = \frac{11 - \sqrt{101}}{2} $$

$$ x = 10.52 , x = 0.48 $$

But, given the constraints of the problem, it seems unlikely that Doug would
finish cleaning the house, by himself, in $0.48$ hours, as he is without Karen.
Additionally, recall that Karen can finish cleaning a house by her self i $x -1$
time, but if we plug in $0.48$ for $x$, we get Karen finishing in $-0.52$ hours,
which doesn't make logical sense. Thusly:

$$ x = 10.52, x \neq 0.48 $$

And therefore, to answer the question of, "How fast can each person clean the
house alone?", we can plug in $10.52$ for x into our original table to get our
answer:

|          | Total Time | Per Hour |
| -------- | ---------- | -------- |
| Doug     | x          | 1/x      |
| Karen    | x - 1      | 1/(x-1)  |
| Together | 5          | 1/5      |

|          | Total Time | Per Hour |
| -------- | ---------- | -------- |
| Doug     | 10.52      | 1/x      |
| Karen    | 9.52       | 1/(x-1)  |
| Together | 5          | 1/5      |

And our answer is:

> Doug can clean the house alone in $10.52$ hours

> Karen can clean the house alone in $9.52$ hours
