# Operations of Functions (Precalculus - College Algebra 5)

[Video](https://www.youtube.com/watch?v=7N_-G4usp6Q)

---

$$ f(x) = \frac{2x + 3}{3x - 2} \quad g(x) = \frac{4x}{3x - 2} $$

$$ \text{D: } \left\{x | \right\} \quad \text{D: } \left\{x | \right\} $$

$$ 3x - 2 = 0 $$

$$ x \neq \frac{2}{3} $$

$$ \text{D: } \left\{x | x \neq \frac{2}{3} \right\} \quad \text{D: } \left\{x | x \neq \frac{2}{3} \right\} $$

---

**Examples:**

---

$$ (f + g)(x) = \left(\frac{2x + 3}{3x - 2}\right) + \left(\frac{4x}{3x - 2}\right) \rightarrow \frac{6x + 3}{3x - 2} $$

$$ \text{D: } \left\{x | x \neq \frac{2}{3} \right\} $$

--

$$ (f - g)(x) = \left(\frac{2x + 3}{3x - 2}\right) - \left(\frac{4x}{3x - 2}\right) \rightarrow \frac{-2x + 3}{3x - 2} $$

Note that the domain is the same as the original, so:

$$ \text{D: } \left\{x | x \neq \frac{2}{3} \right\} $$

---

$$ (f \cdot g)(x) = \left(\frac{2x + 3}{3x - 2}\right) \cdot \left(\frac{4x}{3x - 2}\right) \rightarrow \frac{8x^2 + 12x}{(3x - 2)(3x - 2)} \rightarrow \frac{8x^2 + 12x}{(3x - 2)^2} $$

Note that, once again, we have the same domain:

$$ \text{D: } \left\{x | x \neq \frac{2}{3} \right\} $$

---

$$ \left(\frac{f}{g}\right)(x) = \frac{\dfrac{2x + 3}{3x - 2}}{\dfrac{4x}{3x - 2}} \rightarrow \left(\frac{2x + 3}{3x - 2}\right) \cdot \left(\frac{3x - 2}{4x}\right) \rightarrow \frac{2x + 3}{4x} $$

Note, however, that despite the fact that this _might_ look different, we still
have to write our domain os not including $\dfrac{2}{3}$ first. Our _original_
functions, prior to the composition, basically establish this as a simple fact:

$$ \text{D: } \left\{x | x \neq \frac{2}{3} \right\} $$

Now we can proceed to determine what other numbers our Domain cannot include.

$$ 4x = 0 $$

$$ x \neq 0 $$

$$ \text{D: } \left\{x | x \neq \frac{2}{3} \text{ AND } x \neq 0 \right\} $$

---

$$ f(x) = \sqrt{x + 3} \quad g(x) = \frac{5}{x} $$

$$ \sqrt{x + 3} \geq 0 $$

$$ x + 3 \geq 0 $$

$$ x \geq -3 $$

$$ x \neq 0 $$

$$ \text{D: } \left\{x | x \geq -3 \right\} \quad \text{D: } \left\{x | x \neq 0 \right\} $$

---

$$ (f + g)(x) = \left(\sqrt{x + 3}\right) + \left(\frac{5}{x}\right) $$

$$ \text{D: } \left\{x | x \geq -3 \right\} \quad \text{D: } \left\{x | x \neq 0 \right\} $$

---

$$ (f - g)(x) = \left(\sqrt{x + 3}\right) - \left(\frac{5}{x}\right) $$

$$ \text{D: } \left\{x | x \geq -3 \right\} \quad \text{D: } \left\{x | x \neq 0 \right\} $$

---

$$ (f \cdot g)(x) = \left(\sqrt{x + 3}\right) \cdot \left(\frac{5}{x}\right) $$

$$ \text{D: } \left\{x | x \geq -3 \right\} \quad \text{D: } \left\{x | x \neq 0 \right\} $$

---

$$ \left(\frac{f}{g}\right)(x) = \frac{\left(\sqrt{x + 3}\right)}{\left(\dfrac{5}{x}\right)} \rightarrow \sqrt{x + 3} \cdot \frac{x}{5} \rightarrow \frac{x\sqrt{x + 3}}{5} $$

Notice that this leaves us with a $5$, a _constant_, on the denominator, which
by itself would include _all real numbers_. But we still have to include our
original domains:

$$ \text{D: } \left\{x | x \geq -3 \right\} \quad \text{D: } \left\{x | x \neq 0 \right\} $$
