# Composition of Functions (Precalculus - College Algebra 48)

[Video](https://www.youtube.com/watch?v=EsgHKmLSPVc)

---

We've covered Composite Functions in Intermediate Algebra. In this section,
we're going to go over Composite Functions again in preparation for logarithms
and exponents as the understanding of Composite Functions is related.

In essence, Composite Functions are when one _entire_ function is substituted
into the _variable_ of another function.

---

This is an illustration of the general form you'll see Composite Functions in.

For $f(x)$, $g(x)$:

$$ (f \circ g)(x) = f(g(x)) $$

This is generally said vernacularly as "$f$ of $g$ of $x$". This is essentially
saying, take the entire output from $g(x)$ and plug that in for the input to
$f(x)$.

---

**Examples**

---

Suppose we have these two functions:

$$ f(x) = 2x^2 - 5 $$

$$ g(x) = 1 - 3x^2 $$

So what would the following composite function look like?:

$$ (f \circ g)(x) = \text{?} $$

Essentally we'll take the entire function, $g(x)$ and everywhere there is an $x$
in the function $f(x)$, we'll put the entire function, $g(x)$.

$$ (f \circ g)(x) = 2(1 - 3x^2)^2 - 5 $$

And that really all there is to it.

We can further simplify the function if you like from here, and if we are given
the value of $x$, we can evaluate the function expression.

$$ (f \circ g)(x) = 2(1 - 3x^2)(1 - 3x^2) - 5 $$

$$ (f \circ g)(x) = 2(1 - 6x^2 + 9x^4) - 5 $$

$$ (f \circ g)(x) = 2 - 12x^2 + 18x^4 - 5 $$

$$ (f \circ g)(x) = -12x^2 + 18x^4 - 3 $$

$$ (f \circ g)(x) = 18x^4 -12x^2 - 3 $$

---

Let's take a look at some other examples to really hammer home this point:

$$ (g \circ f)(x) = \text{?} $$

Here we do the same as before, but in reverse. Thusly, we plug in the entire
function $f(x)$ wherever $x$ occurs in $g(x)$:

$$ (g \circ f)(x) = 1 - 3(2x^2 - 5)^2 $$

$$ (g \circ f)(x) = 1 - 3(2x^2 - 5)(2x^2 - 5) $$

$$ (g \circ f)(x) = 1 - 3(4x^4 - 20x^2 + 25) $$

$$ (g \circ f)(x) = 1 - 12x^4 + 60x^2 - 75 $$

$$ (g \circ f)(x) = -12x^4 + 60x^2 - 74 $$

---

What about the same function?

$$ (f \circ f)(x) = \text{?} $$

Well, this is just plugging the original function in for $x$:

$$ (f \circ f)(x) = 2(2x^2 - 5)^2 - 5 $$

$$ (f \circ f)(x) = 2(2x^2 - 5)(2x^2 - 5) - 5 $$

$$ (f \circ f)(x) = 2(4x^4 - 20x^2 + 25) - 5 $$

$$ (f \circ f)(x) = 8x^4 - 40x^2 + 50 - 5 $$

$$ (f \circ f)(x) = 8x^4 - 40x^2 + 45 $$

---

And same if we were to do this for the other function:

$$ (g \circ g)(x) = \text{?} $$

$$ (g \circ g)(x) = 1 - 3(1 - 3x^2)^2 $$

$$ (g \circ g)(x) = 1 - 3(1 - 3x^2)(1 - 3x^2) $$

$$ (g \circ g)(x) = 1 - 3(1 - 6x^2 + 9x^4) $$

$$ (g \circ g)(x) = 1 - 3 + 18x^2 - 27x^4 $$

$$ (g \circ g)(x) = -2 + 18x^2 - 27x^4 $$

$$ (g \circ g)(x) = -27x^4 + 18x^2 - 2 $$

---

Let's now plug in a few values and evaluate:

$$ (f \circ g)(1) = \text{?} $$

Well we can use our previous evaluations of these composite functions to
evaluate this. If we recall we had this for $(f \circ g)(x)$:

$$ (f \circ g)(x) = 2(1 - 3x^2)^2 - 5 $$

So we can just plug in $1$ or simplify and then plug in $1$ and we will get our
answer:

$$ (f \circ g)(1) = 2(1 - 3(1)^2)^2 - 5 $$

$$ (f \circ g)(1) = 2(1 - 3(1))^2 - 5 $$

$$ (f \circ g)(1) = 2(1 - 3)^2 - 5 $$

$$ (f \circ g)(1) = 2(-2)^2 - 5 $$

$$ (f \circ g)(1) = 2(4) - 5 $$

$$ (f \circ g)(1) = 8 - 5 $$

$$ (f \circ g)(1) = 3 $$

---

$$ (g \circ f)(2) = \text{?} $$

$$ (g \circ f)(2) = 1 - 3(2(2)^2 - 5)^2 $$

$$ (g \circ f)(2) = 1 - 3(2(4) - 5)^2 $$

$$ (g \circ f)(2) = 1 - 3(8 - 5)^2 $$

$$ (g \circ f)(2) = 1 - 3(3)^2 $$

$$ (g \circ f)(2) = 1 - 3(9) $$

$$ (g \circ f)(2) = 1 - 27 $$

$$ (g \circ f)(2) = -26 $$

---

$$ (f \circ f)(-1) = \text{?} $$

$$ (f \circ f)(-1) = 2(2(-1)^2 - 5)^2 - 5 $$

$$ (f \circ f)(-1) = 2(2(1) - 5)^2 - 5 $$

$$ (f \circ f)(-1) = 2(2 - 5)^2 - 5 $$

$$ (f \circ f)(-1) = 2(-3)^2 - 5 $$

$$ (f \circ f)(-1) = 2(9) - 5 $$

$$ (f \circ f)(-1) = 18 - 5 $$

$$ (f \circ f)(-1) = 13 $$

---

$$ (g \circ g)(0) = \text{?} $$

$$ (g \circ g)(0) = 1 - 3(1 - 3(0)^2)^2 $$

$$ (g \circ g)(0) = 1 - 3(1 - 3(0))^2 $$

$$ (g \circ g)(0) = 1 - 3(1 - 0)^2 $$

$$ (g \circ g)(0) = 1 - 3(1)^2 $$

$$ (g \circ g)(0) = 1 - 3(1) $$

$$ (g \circ g)(0) = 1 - 3 $$

$$ (g \circ g)(0) = -2 $$
