# How to Find Inverse Trigonometric Functions (Precalculus - Trigonometry 19)

[Video](https://www.youtube.com/watch?v=Ru9Xbd01Jk8)

---

Before diving in on how to find the Inverse Trigonometric Function when given a
Standard Trigonmetric Function given, let's review what we'll need in order to
define an Inverse Trigonometric Function.

Consider the following:

| Trig Function | Domain                                         |
| ------------- | ---------------------------------------------- |
| $\sin x$      | $\left[-\dfrac{\pi}{2}, \dfrac{\pi}{2}\right]$ |
| $\cos x$      | $\left[0, \pi\right]$                          |
| $\tan x$      | $\left(-\dfrac{\pi}{2}, \dfrac{\pi}{2}\right)$ |

Essentially, in order to find the Inverse Trigonometric Function, we must always
Restrict the Domain Of the Trigonometric Function's input, $x$, as defined above
in order to be able to define its Inverse.

In order to find the inverse trigonometric function, we must _Find The Domain
and Range First_. When we evaluate the Inverse Trigonometric Function, we will
find that the Domain and Range of our Original Trigonometric Function switched.

---

$$ f(x) = 5\sin(x) + 2 $$

$$ \text{Domain :} \left\{x \in \R \mid -\frac{\pi}{2} \leq x \leq \frac{\pi}{2} \right\} $$

The Domain is an expression that represents all possible inputs that will give
us a unique output for $f(x)$. In this case, this is the same as the Standard
Sine Domain listed above.

$$ \text{Range: } \left\{f(x) \in \R \mid -3 \leq f(x) \leq 7\right\} $$

The Range is an expression that represents all possible _unique_ outputs that we
can get for $f(x)$. If we evaluate the lowest possible output for $\sin x$, we
get $-1$, and the highest being $1$ (on the Unit Circle). Thusly $\sin x$ will
return $-1$ as its lowest possible value, and $1$ as its highest possible value.
After evalutating $5(-1) + 2$ for our lowest value, and $5(1) + 2$ for our
highest value, we get the Range for $f(x)$.

The next step is to replace our $f(x)$ for $y$:

$$ y = 5\sin(x) + 2 $$

We then swap out our $x$ and $y$ and solve for $y$. Why? Because we are
essentially undoing our entire function and finding the inverse in doing so.

$$ x = 5\sin(y) + 2 $$

$$ x - 2 = 5\sin(y) $$

$$ \frac{x - 2}{5} = \sin(y) $$

$$ \sin^{-1}\left(\frac{x - 2}{5}\right) = \sin^{-1}(\sin(y)) $$

$$ y = \sin^{-1}\left(\frac{x - 2}{5}\right) $$

Now that we've solved for $y$, we will replace it with $f^{-1}(x)$.

$$ f^{-1}(x) = \sin^{-1}\left(\frac{x - 2}{5}\right) $$

Now write out the Range and Domain as switched:

$$ \text{Domain: } \left\{x \in \R \mid -3 \leq x \leq 7\right\} $$

$$ \text{Range:} \left\{f^{-1}(x) \in \R \mid -\frac{\pi}{2} \leq f^{-1}(x) \leq \frac{\pi}{2} \right\} $$

We can also double check if we did this correctly by composing our two
functions, if we did it correctly, it should return back our original input,
$x$:

$$ f(f^{-1}(x)) = 5\sin\left(\sin^{-1}\left(\frac{x - 2}{5}\right)\right) + 2 $$

$$ f(f^{-1}(x)) = 5\cancel{\sin}\left(\cancel{\sin^{-1}}\left(\frac{x - 2}{5}\right)\right) + 2 $$

$$ f(f^{-1}(x)) = 5\left(\frac{x - 2}{5}\right) + 2 $$

$$ f(f^{-1}(x)) = (x - 2) + 2 $$

$$ f(f^{-1}(x)) = x $$

And indeed it does.

---

$$ g(x) = -\tan(x + 1) - 3 $$

$$ \text{Domain: } \left\{(x + 1) \in \R \mid -\frac{\pi}{2} < (x + 1) < \frac{\pi}{2} \right\} $$

This can be more traditionally represented by subtracting $1$ from $x + 1$ and
also on all sides of the inequality:

$$ \text{Domain: } \left\{x \in \R \mid \left(-\frac{\pi}{2} - 1\right) < x < \left(\frac{\pi}{2} - 1\right) \right\} $$

$$ \text{Range: } \left\{g(x) \in \R \mid -\infty < g(x) < \infty \right\} $$

$$ y = -\tan(x + 1) - 3 $$

$$ x = -\tan(y + 1) - 3 $$

$$ x + 3= -\tan(y + 1) $$

$$ -x - 3 = \tan(y + 1) $$

$$ \tan^{-1}(-x - 3) = \tan^{-1}(\tan(y + 1)) $$

$$ y + 1 = \tan^{-1}(-x - 3) $$

$$ y = \tan^{-1}(-x - 3) - 1 $$

$$ g^{-1}(x) = \tan^{-1}(-x - 3) - 1 $$

$$ \text{Domain: } \left\{x \in \R \mid -\infty < x < \infty \right\} $$

$$ \text{Range: } \left\{g^{-1}(x) \in \R \mid \left(-\frac{\pi}{2} - 1\right) < g^{-1}(x) < \left(\frac{\pi}{2} - 1\right) \right\} $$

---

$$ h(x) = 2\cos(3x + 2) - 1 $$

$$ \text{Domain: } \left\{(3x + 2) \in \R \mid 0 \leq (3x + 2) \leq \pi \right\} $$

$$ \text{Domain: } \left\{3x \in \R \mid -2 \leq 3x \leq \pi - 2 \right\} $$

$$ \text{Domain: } \left\{x \in \R \mid -\frac{2}{3} \leq x \leq \frac{\pi - 2}{3} \right\} $$

$$ \text{Range: } \left\{h(x) \in \R \mid -3 \leq h(x) \leq 1 \right\} $$

$$ y = 2\cos(3x + 2) - 1 $$

$$ x = 2\cos(3y + 2) - 1 $$

$$ x + 1 = 2\cos(3y + 2) $$

$$ \frac{x + 1}{2} = \cos(3y + 2) $$

$$ \cos^{-1}\left(\frac{x + 1}{2}\right) = \cos^{-1}(\cos(3y + 2)) $$

$$ 3y + 2 = \cos^{-1}\left(\frac{x + 1}{2}\right) $$

$$ 3y = \cos^{-1}\left(\frac{x + 1}{2}\right) - 2 $$

$$ y = \frac{\cos^{-1}\left(\dfrac{x + 1}{2}\right) - 2}{3} $$

$$ y = \frac{1}{3}\cos^{-1}\left(\dfrac{x + 1}{2}\right) - \frac{2}{3} $$

$$ h^{-1}(x) = \frac{1}{3}\cos^{-1}\left(\dfrac{x + 1}{2}\right) - \frac{2}{3} $$

$$ \text{Domain: } \left\{x \in \R \mid -3 \leq x \leq 1 \right\} $$

$$ \text{Range: } \left\{h^{-1}(x) \in \R \mid -\frac{2}{3} \leq h^{-1}(x) \leq \frac{\pi - 2}{3} \right\} $$
