# How to Prove Trigonometric Identities (Precalculus - Trigonometry 24)

[Video](https://www.youtube.com/watch?v=az_veh1FLbo)

---

As we started to introduce in the previous lecture, there are some recommended
(but not hard rules) steps to simplifying and then evaluating expressions with
Trigonometric Functions with them, and they utilize one or a series of commonly
known, and proven Trigonometric Identities.

In this section, we are going to prove some of these Trigonometric Identities.

Before we get started, however, let us explicitly write out some of these
recommended steps:

1. Start with the "Hard Side" of the Equation

2. Get a Single Fraction

3. Re-write in Sine and Cosine

4. Use _Known_ Identities.

5. Try to work on Just _1 Side_

Also to keep in mind (and possibly memorize) are the _Pythagorean Identities_
(really only the first row is of importance, the others are just different
expressions of the same Identities):

$$ \sin^2\theta + \cos^2\theta = 1 \text{, } \tan^2\theta + 1 = \sec^2\theta \text{, } \cot^2\theta + 1 = \csc^2\theta$$

$$ \sin^2\theta = 1 - \cos^2\theta \text{, } \tan^2\theta = \sec^2\theta - 1 \text{, } \cot^2\theta = \csc^2\theta - 1$$

$$ \cos^2\theta = 1 - \sin^2\theta \text{, } \sec^2\theta - \tan^2\theta = 1 \text{, } \csc^2\theta - \cot^2\theta = 1 $$

---

$$ \sec\theta\sin\theta = \tan\theta $$

When proving Identities, we are provided an Equation, and the only task is to
Prove that indeed, they are the same. In essence, we need to demonstrate this
step by step:

$$ \left(\frac{1}{\cos\theta}\right)\left(\frac{\sin\theta}{1}\right) = \tan\theta $$

$$ \frac{\sin\theta}{\cos\theta} = \tan\theta $$

$$ \tan\theta = \tan\theta $$

---

$$ (\sec\theta -1)(\sec\theta + 1) = \tan^2\theta $$

One might be tempted to "solve" this by setting one side to $0$, but we aren't
Solving, we are Proving, thusly we leave one side untouched (usually the more
simple side of the equation).

$$ (\sec\theta -1)(\sec\theta + 1) = \tan^2\theta $$

$$ \sec^2\theta - 1 = \tan^2\theta $$

If we look at our _Pythagorean Identities_, we'll see that:

$$ \tan^2\theta = \sec^2\theta - 1 $$

Thusly:

$$ \tan^2\theta = \tan^2\theta $$

---

$$ \cos\theta(\tan\theta + \cot\theta) = \csc\theta $$

$$ \cos\theta\left(\frac{\sin\theta}{\cos\theta} + \frac{\cos\theta}{\sin\theta}\right) = \csc\theta $$

$$ \sin\theta + \frac{\cos^2\theta}{\sin\theta} = \csc\theta  $$

$$ \left(\frac{\sin\theta}{\sin\theta}\right)\left(\sin\theta\right) + \frac{\cos^2\theta}{\sin\theta} = \csc\theta  $$

$$ \frac{\sin^2\theta + \cos^2\theta}{\sin\theta} = \csc\theta $$

$$ \frac{1}{\sin\theta} = \csc\theta $$

$$ \csc\theta = \csc\theta $$

---

$$ \sin\theta\csc\theta - \cos^2\theta = \sin^2\theta $$

$$ \left(\frac{\sin\theta}{1}\right)\left(\frac{1}{\sin\theta}\right) - \cos^2\theta = \sin^2\theta $$

$$ 1 - \cos^2\theta = \sin^2\theta $$

And one of our _Pythagorean Identities_ is:

$$ \sin^2\theta = 1 - \cos^2\theta $$

Therefore:

$$ \sin^2\theta = \sin^2\theta $$

---

$$ (1 - \cos^2\theta)(1 + \cot^2\theta) = 1 $$

$$ (\sin^2\theta)(\csc^2\theta) = 1 $$

$$ \left(\frac{\sin^2\theta}{1}\right)\left(\frac{1}{\sin^2\theta}\right) = 1 $$

$$ 1 = 1 $$

---

$$ \sec^4\theta - \sec^2\theta = \tan^4\theta + \tan^2\theta $$

$$ \sec^2\theta(\sec^2\theta - 1) = \tan^4\theta + \tan^2\theta $$

$$ \sec^2\theta(\tan^2\theta) = \tan^4\theta + \tan^2\theta $$

$$ (\tan^2\theta + 1)(\tan^2\theta) = \tan^4\theta + \tan^2\theta $$

$$ \tan^4 + \tan^2\theta = \tan^4\theta + \tan^2\theta $$

---

$$ 3\sin^2\theta + 4\cos^2\theta = 3 + \cos^2\theta $$

$$ 3(1 - \cos^2\theta) + 4\cos^2\theta = 3 + \cos^2\theta $$

$$ 3 - 3\cos^2\theta + 4\cos^2\theta = 3 + \cos^2\theta $$

$$ 3 + \cos^2\theta = 3 + \cos^2\theta $$

---

$$ \frac{\sin^2(-\theta) - \cos^2(-\theta)}{\sin(-\theta) - \cos(-\theta)} = \cos\theta - \sin\theta $$

Let's use Even/Odd Identities to write out our angles without the negatives:

$$ \frac{(-\sin\theta)^2 - (\cos\theta)^2}{-\sin(\theta) - \cos(\theta)} = \cos\theta - \sin\theta $$

$$ \frac{(-1(\sin\theta))^2 - (\cos\theta)^2}{-1(\sin\theta + \cos\theta)} = \cos\theta - \sin\theta $$

$$ \frac{\sin^2\theta - \cos^2\theta}{-1(\sin\theta + \cos\theta)} = \cos\theta - \sin\theta $$

$$ \frac{\sin^2\theta - \cos^2\theta}{-1(\sin\theta + \cos\theta)} = \cos\theta - \sin\theta $$

$$ \left(\frac{-1}{-1}\right)\frac{\sin^2\theta - \cos^2\theta}{-1(\sin\theta + \cos\theta)} = \cos\theta - \sin\theta $$

$$ \frac{-\sin^2\theta + \cos^2\theta}{\sin\theta + \cos\theta} = \cos\theta - \sin\theta $$

$$ \frac{\cos^2\theta - \sin^2\theta}{\sin\theta + \cos\theta} = \cos\theta - \sin\theta $$

$$ \frac{(\cos\theta + \sin\theta)(\cos\theta - \sin\theta)}{\sin\theta + \cos\theta} = \cos\theta - \sin\theta $$

$$ \frac{(\sin\theta + \cos\theta)(\cos\theta - \sin\theta)}{\sin\theta + \cos\theta} = \cos\theta - \sin\theta $$

$$ \frac{\cancel{(\sin\theta + \cos\theta)}(\cos\theta - \sin\theta)}{\cancel{(\sin\theta + \cos\theta)}} = \cos\theta - \sin\theta $$

$$ \cos\theta - \sin\theta = \cos\theta - \sin\theta $$

---

$$ \frac{1 - \cot^2\theta}{1 + \cot^2\theta} + 2\cos^2\theta = 1 $$

$$ \frac{1 - \cot^2\theta}{\csc^2\theta} + 2\cos^2\theta = 1 $$

$$ \frac{1 - \cot^2\theta}{\dfrac{1}{\sin^2\theta}} + 2\cos^2\theta = 1 $$

$$ \sin^2\theta(1 - \cot^2\theta) + 2\cos^2\theta = 1 $$

$$ \sin^2\theta\left(1 - \frac{\cos^2\theta}{\sin^2\theta}\right) + 2\cos^2\theta = 1 $$

$$ \sin^2\theta - \cos^2\theta + 2\cos^2\theta = 1 $$

$$ \sin^2\theta + \cos^2\theta = 1 $$

$$ 1 = 1 $$

---

$$ \frac{1 + \sin\theta}{1 - \sin\theta} - \frac{1 - \sin\theta}{1 + \sin\theta} = 4\tan\theta\sec\theta $$

$$ \left(\frac{1 + \sin\theta}{1 + \sin\theta}\right)\left(\frac{1 + \sin\theta}{1 - \sin\theta}\right) - \left(\frac{1 - \sin\theta}{1 + \sin\theta}\right)\left(\frac{1 - \sin\theta}{1 - \sin\theta}\right) = 4\tan\theta\sec\theta $$

$$ \frac{(1 + \sin\theta)^2 - (1 - \sin\theta)^2}{(1 + \sin\theta)(1 - \sin\theta)} = 4\tan\theta\sec\theta $$

$$ \frac{(1 + \sin\theta)(1 + \sin\theta) - (1 - \sin\theta)(1 - \sin\theta)}{(1 + \sin\theta)(1 - \sin\theta)} = 4\tan\theta\sec\theta $$

$$ \frac{(1 + 2\sin\theta + \sin^2\theta) - (1 - 2\sin\theta + \sin^2\theta)}{(1 + \sin\theta)(1 - \sin\theta)} = 4\tan\theta\sec\theta $$

$$ \frac{1 + 2\sin\theta + \sin^2\theta - 1 + 2\sin\theta - \sin^2\theta}{(1 + \sin\theta)(1 - \sin\theta)} = 4\tan\theta\sec\theta $$

$$ \frac{4\sin\theta}{(1 + \sin\theta)(1 - \sin\theta)} = 4\tan\theta\sec\theta $$

$$ \frac{4\sin\theta}{1 - \sin^2\theta} = 4\tan\theta\sec\theta $$

$$ \frac{4\sin\theta}{\cos^2\theta} = 4\tan\theta\sec\theta $$

$$ \frac{4\sin\theta}{(\cos\theta)(\cos\theta)} = 4\tan\theta\sec\theta $$

$$ 4\left(\frac{\sin\theta}{\cos\theta}\right)\left(\frac{1}{\cos\theta}\right) =  4\tan\theta\sec\theta $$

$$ 4\tan\theta\sec\theta = 4\tan\theta\sec\theta $$

---

$$ \frac{\tan\theta + \sec\theta - 1}{\tan\theta - \sec\theta + 1} = \tan\theta + \sec\theta $$

$$ \frac{\tan\theta + (\sec\theta - 1)}{\tan\theta - (\sec\theta - 1)} = \tan\theta + \sec\theta $$

$$ \left(\frac{\tan\theta + (\sec\theta - 1)}{\tan\theta + (\sec\theta - 1)}\right)\left(\frac{\tan\theta + (\sec\theta - 1)}{\tan\theta - (\sec\theta - 1)}\right) = \tan\theta + \sec\theta $$

$$ \frac{(\tan\theta + (\sec\theta - 1))(\tan\theta + (\sec\theta - 1))}{(\tan\theta + (\sec\theta - 1))(\tan\theta - (\sec\theta  - 1))} = \tan\theta + \sec\theta $$

$$ \frac{\tan^2\theta + 2\tan\theta(\sec\theta - 1) + (\sec\theta - 1)^2}{\tan^2\theta - (\sec\theta - 1)^2} = \tan\theta + \sec\theta $$

$$ \frac{\tan^2\theta + 2\tan\theta(\sec\theta - 1) + (\sec\theta - 1)(\sec\theta - 1)}{\tan^2\theta - (\sec\theta - 1)(\sec\theta - 1)} = \tan\theta + \sec\theta $$

$$ \frac{\tan^2\theta + 2\tan\theta(\sec\theta - 1) + (\sec^2\theta - 2\sec\theta + 1)}{\tan^2\theta - (\sec^2\theta - 2\sec\theta + 1)} = \tan\theta + \sec\theta $$

$$ \frac{\tan^2\theta + 2\tan\theta(\sec\theta - 1) + \sec^2\theta - 2\sec\theta + 1}{\tan^2\theta - \sec^2\theta + 2\sec\theta - 1} = \tan\theta + \sec\theta $$

$$ \frac{(\tan^2\theta + 1) + 2\tan\theta(\sec\theta - 1) + \sec^2\theta - 2\sec\theta}{\tan^2\theta - \sec^2\theta + 2\sec\theta - 1} = \tan\theta + \sec\theta $$

$$ \frac{\sec^2\theta + 2\tan\theta(\sec\theta - 1) + \sec^2\theta - 2\sec\theta}{\tan^2\theta - \sec^2\theta + 2\sec\theta - 1} = \tan\theta + \sec\theta $$

$$ \frac{2\sec^2\theta + 2\tan\theta(\sec\theta - 1) - 2\sec\theta}{\tan^2\theta - \sec^2\theta + 2\sec\theta - 1} = \tan\theta + \sec\theta $$

$$ \frac{2\sec^2\theta + 2\tan\theta(\sec\theta - 1) - 2\sec\theta}{-1(-\tan^2\theta + \sec^2\theta - 2\sec\theta + 1)} = \tan\theta + \sec\theta $$

$$ \frac{2\sec^2\theta + 2\tan\theta(\sec\theta - 1) - 2\sec\theta}{-1((\sec^2\theta - \tan^2\theta) - 2\sec\theta + 1)} = \tan\theta + \sec\theta $$

$$ \frac{2\sec^2\theta + 2\tan\theta(\sec\theta - 1) - 2\sec\theta}{-1((1) - 2\sec\theta + 1)} = \tan\theta + \sec\theta $$

$$ \frac{2\sec^2\theta + 2\tan\theta(\sec\theta - 1) - 2\sec\theta}{-1 + 2\sec\theta - 1} = \tan\theta + \sec\theta $$

$$ \frac{2\sec^2\theta + 2\tan\theta(\sec\theta - 1) - 2\sec\theta}{2\sec\theta - 2} = \tan\theta + \sec\theta $$

$$ \frac{(2\sec^2\theta - 2\sec\theta) + 2\tan\theta(\sec\theta - 1)}{2\sec\theta - 2} = \tan\theta + \sec\theta $$

$$ \frac{2\sec\theta(\sec\theta - 1) + 2\tan\theta(\sec\theta - 1)}{2(\sec\theta - 1)} = \tan\theta + \sec\theta $$

$$ \frac{2\sec\theta\cancel{(\sec\theta - 1)} + 2\tan\theta\cancel{(\sec\theta - 1)}}{2\cancel{(\sec\theta - 1)}} = \tan\theta + \sec\theta $$

$$ \frac{2\sec\theta + 2\tan\theta}{2} = \tan\theta + \sec\theta $$

$$ \frac{\cancel{2}\sec\theta + \cancel{2}\tan\theta}{\cancel{2}} = \tan\theta + \sec\theta $$

$$ \tan\theta + \sec\theta = \tan\theta + \sec\theta $$
