# Introduction to Sum and Difference Formulas in Trigonometry (Precalculus - Trigonometry 25)

[Video](https://www.youtube.com/watch?v=9R5Nz1eYddM)

---

When we find Angles that we need an _Exact_ Solution to, and it's _not_ on the
_Unit Circle_, we can oftentimes use Sum and Difference Forumlas to find said
solution.

Typically, this means that we can add or subtract two different angles using the
standard Trigonometric Functions.

$$ \cos(\alpha + \beta) = \cos\alpha\cos\beta - \sin\alpha\sin\beta $$

$$ \cos(\alpha - \beta) = \cos\alpha\cos\beta + \sin\alpha\sin\beta $$

$$ \sin(\alpha + \beta) = \sin\alpha\cos\beta + \cos\alpha\sin\beta $$

$$ \sin(\alpha - \beta) = \sin\alpha\cos\beta - \cos\alpha\sin\beta $$

$$ \tan(\alpha + \beta) = \frac{\tan\alpha + \tan\beta}{1 - \tan\alpha\tan\beta} $$

$$ \tan(\alpha - \beta) = \frac{\tan\alpha - \tan\beta}{1 + \tan\alpha\tan\beta} $$

Much of the above you see involving $\sin$ and $\cos$ is a _Distance Formula_,
while what you see involving $\tan$ is the comparison of these angles.

---

Let's say we wanted an _Exact_ Solution to the following:

$$ \sin(105\degree) = \text{ ?} $$

It's not on the _Unit Circle_, and we can't just plug it into our calculator, as
that would only give us an _Approximation_. So how do we do this?

If we can take $105\degree$ and break it up into two angles that are on the
_Unit Circle_, then we can represent this as a Sum or Difference of Two angles
and find an _Exact_ Solution.

$$ 105\degree = 60\degree + 45\degree $$

$$ \sin(60\degree + 45\degree) = \text{ ?} $$

We can now take one of our aforementioned sum/difference formulas, specifically:

$$ \sin(\alpha + \beta) = \sin\alpha\cos\beta + \cos\alpha\sin\beta $$

And plug in some values:

$$ \sin(60\degree + 45\degree) = \sin(60\degree)\cos(45\degree) + \cos(60\degree)\sin(45\degree) $$

If we then look at our _Unit Circle_, we can then fill in these values:

$$ \sin(60\degree + 45\degree) = \left(\frac{\sqrt{3}}{2}\right)\left(\frac{\sqrt{2}}{2}\right) + \left(\frac{1}{2}\right)\left(\frac{\sqrt{2}}{2}\right) $$

And now we simply evaluate until we can't anymore (no calculators):

$$ \sin(60\degree + 45\degree) = \left(\frac{\sqrt{3}\sqrt{2}}{4}\right) + \left(\frac{\sqrt{2}}{4}\right) $$

$$ \boxed{\sin(105\degree) = \left(\frac{\sqrt{6} + \sqrt{2}}{4}\right)} $$

This as much as we can simplify our answer, and this represents an _Exact
Solution_ to our original problem statement.

---

$$ \sin\left(\frac{\pi}{12}\right) = \text{ ?} $$

Now, there aren't any two fractions that add up nicely to $\dfrac{\pi}{12}$, the
numerator is pretty small and the denominator is pretty large by comparison to
our Angles represented on the Unit Circle. But two angles do subtract well:

$$ \frac{\pi}{12} = \frac{4\pi}{12} - \frac{3\pi}{12} $$

Why these two angles? Well because when simplified, we can easily see that these
two angles are represented on the Unit Circle:

$$ \frac{\pi}{12} = \frac{\pi}{3} - \frac{\pi}{4} $$

$$ \sin\left(\frac{\pi}{3} - \frac{\pi}{4}\right) = \sin\left(\frac{\pi}{3}\right)\cos\left(\frac{\pi}{4}\right) - \cos\left(\frac{\pi}{3}\right)\sin\left(\frac{\pi}{4}\right)$$

$$ \sin\left(\frac{\pi}{3} - \frac{\pi}{4}\right) = \left(\frac{\sqrt{3}}{2}\right)\left(\frac{\sqrt{2}}{2}\right) - \left(\frac{1}{2}\right)\left(\frac{\sqrt{2}}{2}\right)$$

$$ \boxed{\sin\left(\frac{\pi}{12}\right) = \frac{\sqrt{6} - \sqrt{2}}{4}} $$

---

$$ \cos(165\degree) = \text{ ?} $$

The general idea behind evaluating whether to add or subtract does have to do
with how large of an angle are we talking? If it is a very small angle, like a
fraction of a radian, then we would subtract, if it is a large angle, like this
one, we likely want to add. This is not a hard rule, it is just something to
keep in mind as it generally helps.

$$ 165\degree = 120\degree + 45\degree $$

Both $120\degree$ and $45\degree$ lie on the _Unit Circle_. We can now
substitute these angles into the formula for addition of Cosine:

$$ \cos(\alpha + \beta) = \cos\alpha\cos\beta - \sin\alpha\sin\beta $$

$$ \cos(120\degree + 45\degree) = \cos(120\degree)\cos(45\degree)- \sin(120\degree)\sin(45\degree) $$

$$ \cos(120\degree + 45\degree) = \left(-\frac{1}{2}\right)\left(\frac{\sqrt{2}}{2}\right) - \left(\frac{\sqrt{3}}{2}\right)\left(\frac{\sqrt{2}}{2}\right) $$

$$ \cos(120\degree + 45\degree) = -\frac{\sqrt{2}}{4} - \frac{\sqrt{6}}{4} $$

$$ \boxed{\cos(165\degree) = \frac{-\sqrt{2} - \sqrt{6}}{4}} $$

Note that you could have solved this using $135\degree$ and $30\degree$ angles
as those also lie on the Unit Circle.

---

$$ \tan\left(\frac{19\pi}{12}\right) = \text{ ?} $$

This is a rather large angle, we should probably go for an addition.

$$ \frac{19\pi}{12} = \frac{16\pi}{12} + \frac{3\pi}{12} $$

$$ \frac{19\pi}{12} = \frac{4\pi}{3} + \frac{\pi}{4} $$

$$ \tan\left(\frac{4\pi}{3} + \frac{\pi}{4}\right) = \text{ ?} $$

Now we just need our Tangent Addition Formula:

$$ \tan(\alpha + \beta) = \frac{\tan\alpha + \tan\beta}{1 - \tan\alpha\tan\beta} $$

$$ \tan\left(\frac{4\pi}{3} + \frac{\pi}{4}\right) = \frac{\tan\left(\dfrac{4\pi}{3}\right) + \tan\left(\dfrac{\pi}{4}\right)}{1 - \tan\left(\dfrac{4\pi}{3}\right)\tan\left(\dfrac{\pi}{4}\right)}$$

And now evaluate:

$$ \tan\left(\frac{19\pi}{12}\right) = \frac{\sqrt{3} + 1}{1 - \sqrt{3}} $$

You can rationalize the denominator by multiplying by something that will give
you a difference of squares:

$$ \tan\left(\frac{19\pi}{12}\right) = \frac{\sqrt{3} + 1}{1 - \sqrt{3}} \cdot \frac{1 + \sqrt{3}}{1 + \sqrt{3}} $$

$$ \tan\left(\frac{19\pi}{12}\right) = \frac{1 + 2\sqrt{3} + 3}{1 - 3} $$

$$ \tan\left(\frac{19\pi}{12}\right) = -\frac{4 + 2\sqrt{3}}{2} $$

$$ \boxed{\tan\left(\frac{19\pi}{12}\right) = -2 - \sqrt{3}} $$

---

$$ \tan(15\degree) = \text{ ?} $$

This is a very small angle, it's even smaller than our smallest angle on the
Unit Circle ($30\degree$), so we'll likely need subtraction to solve this.

$$ 15\degree = 45\degree - 30\degree $$

Now we just need our Tangent Difference Formula:

$$ \tan(\alpha - \beta) = \frac{\tan\alpha - \tan\beta}{1 + \tan\alpha\tan\beta} $$

$$ \tan(45\degree - 30\degree) = \frac{\tan(45\degree) - \tan(30\degree)}{1 + \tan(45\degree)\tan(30\degree)} $$

$$ \tan(45\degree - 30\degree) = \frac{1 - \dfrac{\sqrt{3}}{3}}{1 + \dfrac{\sqrt{3}}{3}} $$

And we can rationalize this further:

$$ \tan(45\degree - 30\degree) = \frac{1 - \dfrac{\sqrt{3}}{3}}{1 + \dfrac{\sqrt{3}}{3}} \cdot \frac{1 - \dfrac{\sqrt{3}}{3}}{1 - \dfrac{\sqrt{3}}{3}} $$

$$ \tan(45\degree - 30\degree) = \frac{1 - \dfrac{2\sqrt{3}}{3} + \dfrac{1}{3}}{1 - \dfrac{1}{3}}$$

$$ \tan(45\degree - 30\degree) = \frac{1 - \dfrac{2\sqrt{3}}{3} + \dfrac{1}{3}}{\dfrac{2}{3}}$$

$$ \tan(45\degree - 30\degree) = \left(1 - \dfrac{2\sqrt{3}}{3} + \dfrac{1}{3}\right) \cdot \frac{3}{2} $$

$$ \tan(45\degree - 30\degree) = \frac{3}{2} - \sqrt{3} + \frac{1}{2} $$

$$ \boxed{\tan(15\degree) = 2 - \sqrt{3}} $$

---

$$ \sec\left(-\frac{\pi}{12}\right) = \text{ ?} $$

Because Secant is an _Even_ Function, we can change the sign of the argument
without problematic consequences:

$$ \sec\left(-\frac{\pi}{12}\right) \rightarrow \sec\left(\frac{\pi}{12}\right) = \text{ ?} $$

Because $\dfrac{\pi}{12}$ is a very small angle, smaller than our smallest Unit
Circle Angle of $\dfrac{\pi}{6}$, we probably will use subtraction to parse out
our angle:

$$ \frac{\pi}{12} = \frac{3\pi}{12} - \frac{2\pi}{12} $$

$$ \frac{\pi}{12} = \frac{\pi}{4} - \frac{\pi}{6} $$

$$ \sec\left(\frac{\pi}{4} - \frac{\pi}{6}\right) = \text{ ?} $$

Now, Secant is not represented by our standard Sum and Difference Formulas, but
if we take the Cosecant of this angle, find it, and then take the Reciprocal, we
will find the Secant.

$$ \sec\left(\frac{\pi}{4} - \frac{\pi}{6}\right) = \frac{1}{\cos\left(\dfrac{\pi}{4} - \dfrac{\pi}{6}\right)} $$

Let's therefore find the Cosecant:

$$ \cos\left(\frac{\pi}{4} - \frac{\pi}{6}\right) = \text{ ?} $$

The standard Cosecant subtraction formula is:

$$ \cos(\alpha - \beta) = \cos\alpha\cos\beta + \sin\alpha\sin\beta $$

$$ \cos\left(\frac{\pi}{4} - \frac{\pi}{6}\right) = \cos\left(\frac{\pi}{4}\right)\cos\left(\frac{\pi}{6}\right) + \sin\left(\frac{\pi}{4}\right)\sin\left(\frac{\pi}{6}\right) $$

$$ \cos\left(\frac{\pi}{4} - \frac{\pi}{6}\right) = \left(\frac{\sqrt{2}}{2}\right)\left(\frac{\sqrt{3}}{2}\right) + \left(\frac{\sqrt{2}}{2}\right)\left(\frac{1}{2}\right)$$

$$ \cos\left(\frac{\pi}{4} - \frac{\pi}{6}\right) = \frac{\sqrt{6} + \sqrt{2}}{4} $$

$$ \sec\left(\frac{\pi}{4} - \frac{\pi}{6}\right) = \frac{4}{\sqrt{6} + \sqrt{2}} $$

Now we rationalize:

$$ \sec\left(\frac{\pi}{4} - \frac{\pi}{6}\right) = \frac{4}{\sqrt{6} + \sqrt{2}} \cdot \frac{\sqrt{6} - \sqrt{2}}{\sqrt{6} - \sqrt{2}} $$

$$ \sec\left(\frac{\pi}{4} - \frac{\pi}{6}\right) = \frac{4\sqrt{6} - 4\sqrt{2}}{6 - 2} $$

$$ \sec\left(\frac{\pi}{4} - \frac{\pi}{6}\right) = \frac{4\sqrt{6} - 4\sqrt{2}}{4} $$

$$ \sec\left(\frac{\pi}{4} - \frac{\pi}{6}\right) = \sqrt{6} - \sqrt{2} $$

$$ \boxed{\sec\left(-\frac{\pi}{12}\right) = \sqrt{6} - \sqrt{2}} $$

---

Now let's see what it's like to do this in reverse:

$$ \sin(20\degree)\cos(80\degree) - \cos(20\degree)\sin(80\degree) $$

This is the same as:

$$ \sin(\alpha - \beta) = \sin\alpha\cos\beta - \cos\alpha\sin\beta $$

$$ \sin(20\degree)\cos(80\degree) - \cos(20\degree)\sin(80\degree) = \sin(20\degree - 80\degree) = \sin(-60\degree) $$

Recall that Sine is an _Odd_ Function:

$$ \sin(-\theta) = -\sin\theta $$

Therefore:

$$ \sin(-60\degree) = -\sin(60\degree) $$

And $\sin(60\degree) = \dfrac{\sqrt{3}}{2}$, while $-\sin(60\degree) =
-\dfrac{\sqrt{3}}{2}$.

Therefore:

$$ \boxed{\sin(20\degree)\cos(80\degree) - \cos(20\degree)\sin(80\degree) = -\frac{\sqrt{3}}{2}} $$

---

$$ \frac{\tan(40\degree) - \tan(10\degree)}{1 + \tan(40\degree)\tan(10\degree)} $$

$$ \tan(\alpha - \beta) = \frac{\tan\alpha - \tan\beta}{1 + \tan\alpha\tan\beta} $$

$$ \frac{\tan(40\degree) - \tan(10\degree)}{1 + \tan(40\degree)\tan(10\degree)} = \tan(30\degree) $$

$$ \tan(30\degree) = \frac{\sqrt{3}}{3} $$

$$ \boxed{\frac{\tan(40\degree) - \tan(10\degree)}{1 + \tan(40\degree)\tan(10\degree)} = \frac{\sqrt{3}}{3}} $$

---

$$ \sin\left(\frac{\pi}{12}\right)\cos\left(\frac{7\pi}{12}\right) - \cos\left(\frac{\pi}{12}\right)\sin\left(\frac{7\pi}{12}\right) $$

$$ \sin(\alpha - \beta) = \sin\alpha\cos\beta - \cos\alpha\sin\beta $$

$$ \sin\left(\frac{\pi}{12}\right)\cos\left(\frac{7\pi}{12}\right) - \cos\left(\frac{\pi}{12}\right)\sin\left(\frac{7\pi}{12}\right) = \sin\left(-\frac{6\pi}{12}\right) $$

$$ \sin(-\theta) = -\sin\theta $$

$$ \sin\left(-\frac{6\pi}{12}\right) = -\sin\left(\frac{6\pi}{12}\right) = -\sin\left(\frac{\pi}{2}\right) = -1 $$

$$ \boxed{\sin\left(\frac{\pi}{12}\right)\cos\left(\frac{7\pi}{12}\right) - \cos\left(\frac{\pi}{12}\right)\sin\left(\frac{7\pi}{12}\right) = -1} $$
