# How to Convert From Polar Equations to Rectangular Equations (Precalculus - Trigonometry 40)

[Video](https://www.youtube.com/watch?v=QjU4_fO8V2I)

---

In the previous lecture, we went over how to convert Rectangular Equations To
Polar Equations. In this lecture, we will do the opposite, converting from Polar
Equations To Rectangular Equations:

Recall these formulas from the previous lecture:

$$ x^2 + y^2 = r^2 $$

$$ x = r\cos\theta $$

$$ y = r\sin\theta $$

A lot of today's lecture will demonstrate that these same formulas can help us
converting Polar Coordinates To Rectangular Coordinates.

---

Consider the following Polar Coordinate Equation:

$$ r = \cos\theta $$

We don't really have anything here that resembes our formulas above, but we can
get closer by simply multiplying both sides of our equation by $r$:

$$ r^2 = r\cos\theta $$

And now we do have a couple things that look familiar:

$$ x^2 + y^2 = x $$

And this is actually all we have to do.

---

Consider the following Polar Coordinate Equation:

$$ r = \sin\theta + 1 $$

$$ r \cdot r = (\sin\theta + 1) \cdot r $$

$$ r^2 = r\sin\theta + r $$

$$ x^2 + y^2 = y + r $$

$$ \boxed{x^2 + y^2 = y + \sqrt{x^2 + y^2}} $$

Note how the original Polar looks a bit easier to reason about.

---

Consider the following Polar Coordinate Equation:

$$ r^2 = \cos\theta $$

$$ r \cdot r^2 = r\cos\theta $$

$$ \sqrt{x^2 + y^2}(x^2 + y^2) = x $$

$$ (x^2 + y^2)^{\frac{1}{2}}(x^2 + y^2)^1 = x $$

$$ (x^2 + y^2)^{\frac{3}{2}} = x $$

---

Consider the following Polar Coordinate Equation:

$$ r = \frac{\sin\theta}{\cos^2\theta} $$

$$ \cos\theta \cdot r = \frac{\sin\theta}{\cos\theta} \cdot \frac{1}{\cos\theta} \cdot \cos\theta $$

$$ r\cos\theta = \tan\theta $$

$$ x = \frac{y}{x} $$

$$ y = x^2 $$

---

Consider the following Polar Coordinate Equation:

$$ r = 3\csc\theta $$

$$ r = \frac{3}{\sin\theta} $$

$$ \sin\theta \cdot r = \frac{3}{\sin\theta} \cdot \sin\theta $$

$$ r\sin\theta = 3 $$

$$ y = 3 $$

---

Consider the following Polar Coordinate Equation:

$$ r = \sin\theta\cos^2\theta $$

$$ r^3 \cdot r = \sin\theta\cos^2\theta \cdot r^3 $$

$$ r^4 = r\sin\theta \cdot r\cos\theta \cdot r\cos\theta $$

$$ (x^2 + y^2)^2 = x^2y $$

$$ \sqrt{(x^2 + y^2)^2} = \sqrt{x^2y} $$

$$ x^2 + y^2 = x\sqrt{y} $$

---

Consider the following Polar Coordinate Equation:

$$ r = 2 $$

$$ \sqrt{x^2 + y^2} = 2 $$

$$ (\sqrt{x^2 + y^2})^2 = (2)^2 $$

$$ x^2 + y^2 = 4 $$

---

Consider the following Polar Coordinate Equation:

$$ r = \frac{4}{1 - \cos\theta} $$

$$ r(1 - \cos\theta) = 4 $$

$$ r - r\cos\theta = 4 $$

$$ \sqrt{x^2 + y^2} - x = 4 $$

$$ \sqrt{x^2 + y^2} = 4 + x $$

$$ (\sqrt{x^2 + y^2})^2 = (x + 4)^2 $$

$$ x^2 + y^2 = x^2 + 8x + 16 $$

$$ y^2 = 8x + 16 $$

$$ y^2 - 8x - 16 = 0 $$
